%============================================================================
% Daniel J. Greenhoe
% LaTeX file
%============================================================================
%============================================================================
\subsection{Case study: Parallel operators}
%============================================================================
%---------------------------------------
\begin{minipage}{\tw-70mm}
\begin{proposition}
\label{prop:xGw_xHy}
%---------------------------------------
Let $\opS$ be the \structe{system} illustrated to the right,
where $\opT$ is \prope{not necessarily linear}.
Let 
\\\indentx$\ds\seqn{\fh(n)}\eqd\opH\kdelta(n)\eqd\sum_{m\in\Z}\fh(m)\kdelta(n-m)$
\\
be the \fncte{impulse response} of $\opH$.
\end{proposition}
\end{minipage}
\hfill\tbox{\includegraphics{graphics/xTy_xHw.pdf}}
\\
\propbox{
  \brb{\begin{array}{FMMD}
      (A).& $\rvx(n)$ is &\prope{WSS}       & and
    \\(B).& $\opH$    is &\prope{LTI}       &
  \end{array}}
  \implies
  \brb{\begin{array}{lc  >{\ds}l             @{\hspace{1pt}}l  M                     D}
      \Szwy(z)       &=& \ZH(z)              &\Szxy(z)       & for (1),(3),(5),(6) & and
    \\\Swwy(\omega)  &=& \FH(\omega)         &\Swxy(\omega)  & for (1),(3),(5),(6) & and
    \\\hline
      \Szwy(z)       &=& \ZH^\ast\brp{z^\ast}&\Szxy(z)       & for (2),(4),(7),(8) & and
    \\\Swwy(\omega)  &=& \FH^\ast(-\omega)   &\Swxy(\omega)  & for (2),(4),(7),(8) & 
  \end{array}}
  }
\\
\begin{proof}
\begin{align*}
  (1).\quad\Rwy(m)
    &\eqd \pE\brs{\rvw(m)\rvy^\ast(0)}
    && \text{by (A) and Papoulis' definition of $\Rwy$}
    && \text{\xref{def:Rxym}}
  \\&\eqd \pE\brp{\brs{\opH\rvx}(m)\rvy^\ast(0)}
    && \text{by definition of $\opS$}
  \\&= \opH\pE\brp{\rvx(m)\rvy^\ast(0)}
    && \text{by \prope{LTI} hypothesis}
    && \text{(B)}
  \\&\eqd \opH\Rxy(m)
    && \text{by Papoulis' definition of $\Rwy$}
    && \text{\xref{def:Rxym}}
  \\&= \sum_{n\in\Z}\fh(n)\Rxy(m-n)
    && \mathrlap{\text{by definition of \fncte{impulse response} $\seqn{\fh(n)}$}}
  \\&= \brs{\fh\convd\Rxy}(m)
    && \text{by definition of \ope{convolution}}
    && \text{\xref{def:dsp_conv}}
\end{align*}

\begin{align*}
    (2).\quad\Rwy(m)
      &\eqd \pE\brs{\rvw^\ast(0)\rvy(m)}
     &&\eqd \pE\brp{\brs{\opH\rvx}^\ast(0)\rvy(m)}
     &&=    \opH^\ast\brp{\pE\brs{\rvx^\ast(0)\rvy(m)}}
     &&\eqd \opH^\ast\Rxy(m)
     &&=    \brs{\fh^\ast\convd\Rxy}(m)
     \\
    (3).\quad\Rwy(m)
      &\eqd \pE\brs{\rvw(0)\rvy^\ast(m)}
     &&\eqd \pE\brp{\brs{\opH\rvx}(0)\rvy^\ast(m)}
     &&=    \opH\brp{\pE\brs{\rvx(0)\rvy^\ast(m)}}
     &&\eqd \opH\Rxy(m)
     &&=    \brs{\fh\convd\Rxy}(m)
     \\
    (4).\quad\Rwy(m)
      &\eqd \pE\brs{\rvw^\ast(m)\rvy(0)}
     &&\eqd \pE\brp{\brs{\opH\rvx}^\ast(m)\rvy(0)}
     &&=    \opH^\ast\brp{\pE\brs{\rvx^\ast(m)\rvy(0)}}
     &&\eqd \opH^\ast\Rxy(m)
     &&=    \brs{\fh^\ast\convd\Rxy}(m)
     \\
    (5).\quad\Rwy(m)
      &\eqd \pE\brs{\rvw(0)\rvy(m)}
     &&\eqd \pE\brp{\brs{\opH\rvx}(0)\rvy(m)}
     &&=    \opH\brp{\pE\brs{\rvx(0)\rvy(m)}}
     &&\eqd \opH\Rxy(m)
     &&=    \brs{\fh\convd\Rxy}(m)
     \\
    (6).\quad\Rwy(m)
      &\eqd \pE\brs{\rvw(m)\rvy(0)}
     &&\eqd \pE\brp{\brs{\opH\rvx}(m)\rvy(0)}
     &&=    \opH\brp{\pE\brs{\rvx(m)\rvy(0)}}
     &&\eqd \opH\Rxy(m)
     &&=    \brs{\fh\convd\Rxy}(m)
    \\
    (7).\quad\Rwy(m)
      &\eqd \pE\brs{\rvw^\ast(0)\rvy^\ast(m)}
     &&\eqd \pE\brp{\brs{\opH\rvx}^\ast(0)\rvy^\ast(m)}
     &&=    \opH^\ast\brp{\pE\brs{\rvx^\ast(0)\rvy^\ast(m)}}
     &&\eqd \opH^\ast\Rxy(m)
     &&=    \brs{\fh^\ast\convd\Rxy}(m)
    \\
    (8).\quad\Rwy(m)
      &\eqd \pE\brs{\rvw^\ast(m)\rvy^\ast(0)}
     &&\eqd \pE\brp{\brs{\opH\rvx}^\ast(m)\rvy^\ast(0)}
     &&=    \opH^\ast\brp{\pE\brs{\rvx^\ast(m)\rvy^\ast(0)}}
     &&\eqd \opH^\ast\Rxy(m)
     &&=    \brs{\fh^\ast\convd\Rxy}(m)
\end{align*}
\begin{align*}
  (1),(3),(5),(6).\quad\Szwy(z)
    &\eqd \opZ\Rwy(m)
   &&= \opZ\brs{\fh\convd\Rxy}(m)
   &&= \ZH(z)\Szxy(z)
  \\
  (2),(4),(7),(8).\quad\Szwy(z)
    &\eqd \opZ\Rwy(m)
   &&= \opZ\brs{\fh^\ast\convd\Rxy}(m)
   &&= \ZH^\ast\brp{z^\ast}\Szxy(z)
   && \text{by \prefp{prop:opZ}}
  \\
  (1),(3),(5),(6).\quad\Swwy(\omega)
    &\eqd \opDTFT\Rwy(m)
   &&= \opDTFT\brs{\fh\convd\Rxy}(m)
   &&= \FH(\omega)\Swxy(\omega)
  \\
  (2),(4),(7),(8).\quad\Swwy(\omega)
    &\eqd \opDTFT\Rwy(m)
   &&= \opDTFT\brs{\fh^\ast\convd\Rxy}(m)
   &&= \FH^\ast(-\omega)\Swxy(\omega)
   && \text{by \prefp{prop:opZ}}
\end{align*}
\end{proof}

