%============================================================================
% Daniel J. Greenhoe
% LaTeX file
%============================================================================
%============================================================================
\subsection{Case study: Linear system identification}
%============================================================================
%=======================================
%\subsection{Least squares estimates of linear systems}
%=======================================
\begin{figure}
  \centering
  \tbox{\includegraphics{graphics/opH_mnoise.pdf}}
  \caption{Additive noise linear system for \pref{sec:case_estHx} Case study (System identification)\label{fig:addnoise_LTI}}
\end{figure}

% ___________________________________________________________________________________
%| |                                   ____________________________________________  |
%|D|                               \  /[                   ]2          |        |2   |
%|E|          Syy(w) - k(w)Sxx(w) + \/ [Syy(w) - k(w)Sxx(w)]   + 4 k(w)| Sxy(w) |    |
%|F| Hk(w) = --------------------------------------- ----------------- ------------- |
%| |                                       2 Sxy(w)                                  |
%|_|_________________________________________________________________________________|
\begin{definition}                                                                   %
\footnote{                                                                           %
  \citePpc{white2006}{679}{(6)},                                                     %
  \citerpgc{shin2008}{293}{0470725648}{(9.67)},                                      %
  \citePpc{wicks1986}{898}{has additional $s$ in denominator}
  }                                                                                  %
\label{def:Hkp}                                                                      %
%------------------------------------------------------------------------------------%
Let $\opS$ be the \structe{system} illustrated in \prefpp{fig:addnoise_LTI}.
\defbox{\begin{array}{l>{\ds}rc>{\ds}lC}
  \mc{5}{M}{
  The \fnctd{transfer function estimate $\estHkp(\omega; \kappa)$}
  with \vald{scaling function} $\kappa(\omega)$ is defined as
  }
  \\&
  \estHkp(\omega; \kappa) &\eqd&
      \frac{\Swyy(\omega)-\kappa(\omega)\Swxx(\omega) +
            \sqrt{\brs{\Swyy(\omega) - \kappa(\omega)\Swxx(\omega)}^2 +
                  4\kappa(\omega)\abs{\Swxy(\omega)}^2}
           }
           {2\Swxy(\omega)}
    & \forall \omega,\kappa(\omega)\in\R
  \\
  \mc{5}{M}{The \fnctd{transfer function estimate $\estHs(\omega; s)$}
  with \vald{scaling constant} $s$ is defined as}
  \\&
  \estHs(\omega; s) &\eqd& \brlr{\estHkp(\omega; \kappa)}_{\kappa=s^2}
    & \forall \omega,s\in\R
\end{array}}
\end{definition}

%---------------------------------------
\begin{lemma}
\label{lem:estHk_Suu}
%---------------------------------------
Let $\opS$ be the \structe{system} illustrated in \prefpp{fig:addnoise_LTI}.
\lemboxt{
  $\brb{\begin{array}{M}
           There exists $\kappa(\omega)$ such that
         $\Swvv(\omega)=\kappa(\omega)\Swuu(\omega)$
  \end{array}}$
  \\\indentx$\implies
  \brb{\begin{array}{>{\ds}rc>{\ds}l}
    \Swuu(\omega) = \frac{\abs{\estH(\omega)}^2\Swxx(\omega) - \estH(\omega)\Swxy(\omega) - \estH^\ast(\omega)\Swxy^\ast(\omega) + \Swyy(\omega)}
                         {\kappa(\omega)+\abs{\estH(\omega)}^2}
  \end{array}}$
  }
\end{lemma}
\begin{proof}
\begin{align*}
     (1).\quad \Swuu(\omega) &= \Swxx(\omega) - \Swpp(\omega) &&=\ocom{\Swxx(\omega) - \frac{\Swpq(\omega)}{\estH^\ast( \omega)}}{by \pref{cor:RxySwxy}} &&= \ocom{\Swxx(\omega) - \frac{\Swxy(\omega)}{\estH^\ast( \omega)}}{by \prope{uncorrelated} hypothesis}
  %\\(2).\quad \Swuu(\omega) &= \Swxx(\omega) - \Swpp(\omega) &&= \Swxx(\omega) - \ffrac{\Swpq(\omega)}{\estH     ( \omega)} &&= \Swxx(\omega) - \ffrac{\Swxy(\omega)}{\estH     ( \omega)}
  %\\(3).\quad \Swuu(\omega) &= \Swxx(\omega) - \Swpp(\omega) &&= \Swxx(\omega) - \ffrac{\Swpq(\omega)}{\estH^\ast(-\omega)} &&= \Swxx(\omega) - \ffrac{\Swxy(\omega)}{\estH^\ast(-\omega)}
  %\\(4).\quad \Swuu(\omega) &= \Swxx(\omega) - \Swpp(\omega) &&= \Swxx(\omega) - \ffrac{\Swpq(\omega)}{\estH     (-\omega)} &&= \Swxx(\omega) - \ffrac{\Swxy(\omega)}{\estH     (-\omega)}
  %\\(5).\quad \Swuu(\omega) &= \Swxx(\omega) - \Swpp(\omega) &&= \Swxx(\omega) - \ffrac{\Swpq(\omega)}{\estH     ( \omega)} &&= \Swxx(\omega) - \ffrac{\Swxy(\omega)}{\estH     ( \omega)}
  %\\(6).\quad \Swuu(\omega) &= \Swxx(\omega) - \Swpp(\omega) &&= \Swxx(\omega) - \ffrac{\Swpq(\omega)}{\estH     (-\omega)} &&= \Swxx(\omega) - \ffrac{\Swxy(\omega)}{\estH     (-\omega)}
  %\\(7).\quad \Swuu(\omega) &= \Swxx(\omega) - \Swpp(\omega) &&= \Swxx(\omega) - \ffrac{\Swpq(\omega)}{\estH^\ast(-\omega)} &&= \Swxx(\omega) - \ffrac{\Swxy(\omega)}{\estH^\ast(-\omega)}
  %\\(8).\quad \Swuu(\omega) &= \Swxx(\omega) - \Swpp(\omega) &&= \Swxx(\omega) - \ffrac{\Swpq(\omega)}{\estH     (-\omega)} &&= \Swxx(\omega) - \ffrac{\Swxy(\omega)}{\estH     (-\omega)}
  %\\
   \\(1).\quad \Swvv(\omega) &= \Swyy(\omega) - \Swqq(\omega) &&= \Swyy(\omega) - \Swpq(\omega)\estH     ( \omega) &&= \Swyy(\omega) - \Swxy(\omega)\estH     ( \omega)
  %\\(2).\quad \Swvv(\omega) &= \Swyy(\omega) - \Swqq(\omega) &&= \Swyy(\omega) - \Swpq(\omega)\estH     ( \omega) &&= \Swyy(\omega) - \Swxy(\omega)\estH     ( \omega)
  %\\(3).\quad \Swvv(\omega) &= \Swyy(\omega) - \Swqq(\omega) &&= \Swyy(\omega) - \Swpq(\omega)\estH     (-\omega) &&= \Swyy(\omega) - \Swxy(\omega)\estH     (-\omega)
  %\\(4).\quad \Swvv(\omega) &= \Swyy(\omega) - \Swqq(\omega) &&= \Swyy(\omega) - \Swpq(\omega)\estH^\ast(-\omega) &&= \Swyy(\omega) - \Swxy(\omega)\estH^\ast(-\omega)
  %\\(5).\quad \Swvv(\omega) &= \Swyy(\omega) - \Swqq(\omega) &&= \Swyy(\omega) - \Swpq(\omega)\estH     (-\omega) &&= \Swyy(\omega) - \Swxy(\omega)\estH     (-\omega)
  %\\(6).\quad \Swvv(\omega) &= \Swyy(\omega) - \Swqq(\omega) &&= \Swyy(\omega) - \Swpq(\omega)\estH     ( \omega) &&= \Swyy(\omega) - \Swxy(\omega)\estH     ( \omega)
  %\\(7).\quad \Swvv(\omega) &= \Swyy(\omega) - \Swqq(\omega) &&= \Swyy(\omega) - \Swpq(\omega)\estH     ( \omega) &&= \Swyy(\omega) - \Swxy(\omega)\estH     ( \omega)
  %\\(8).\quad \Swvv(\omega) &= \Swyy(\omega) - \Swqq(\omega) &&= \Swyy(\omega) - \Swpq(\omega)\estH     ( \omega) &&= \Swyy(\omega) - \Swxy(\omega)\estH     ( \omega)
%  \\
%  \\(1).\quad \Swuu\brs{\abs{\estH}^2+\kappa} &= \Swuu\abs{\estH}^2 + \Swvv &&= \abs{\estH}^2\brs{\Swxx - \frac{\Swxy}{\estH^\ast}} +\brs{\Swyy - \Swxy\estH}  &&= \abs{\estH}^2\Swxx - \estH^\ast\Swyx -\Swxy\estH + \Swyy
%  \\
\end{align*}

\begin{align*}
    (1).\quad \Swuu\brs{\abs{\estH}^2+\kappa}
          &= \Swuu\abs{\estH}^2 + \Swvv
         &&= \abs{\estH}^2\brs{\Swxx - \frac{\Swxy}{\estH^\ast}} +\brs{\Swyy - \Swxy\estH}
         &&= \abs{\estH}^2\Swxx - 2\estH\Swxy + \Swyy
    \\
    (2).\quad \Swuu\brs{\abs{\estH}^2+\kappa}
         &= \Swuu\abs{\estH}^2 + \Swvv
         &&= \abs{\estH}^2\brs{\Swxx - \frac{\Swxy}{\estH}} +\brs{\Swyy - \Swxy\estH}
         &&= \abs{\estH}^2\Swxx - \estH^\ast\Swxy - \estH\Swxy + \Swyy
    \\
    (3).\quad \Swuu\brs{\abs{\estH}^2+\kappa}
          &= \Swuu\abs{\estH}^2 + \Swvv
         &&= \abs{\estH}^2\brs{\Swxx - \frac{\Swxy}{\estH^\ast(-\omega)}} +\brs{\Swyy - \Swxy\estH(-\omega)}
        % &&= \abs{\estH}^2\Swxx - \estH^\ast\Swxy - \estH\Swxy + \Swyy 
\end{align*}

\begin{align*}
     \Swuu\brs{\abs{\estH}^2+\kappa}
          &= \abs{\estH}^2\Swuu +\kappa\Swuu
          && \eqd \Swuu\abs{\estH}^2 + \Swvv
          &&= \abs{\estH}^2\brs{\Swxx - \frac{\Swyx}{\estH}}
      +\brs{\Swyy - \Swxy\estH}
  \\&= \abs{\estH}^2\Swxx - \estH^\ast\Swyx
      -\Swxy\estH + \Swyy
  \\&\mathrlap{\implies
    \boxed{
      \Swuu(\omega) = \frac{\abs{\estH(\omega)}^2\Swxx(\omega) - \estH(\omega)\Swxy(\omega) - \estH^\ast(\omega)\Swxy^\ast(\omega) + \Swyy(\omega)}
                   {\kappa(\omega)+\abs{\estH(\omega)}^2}
            }}
\end{align*}
\end{proof}

%---------------------------------------
\begin{theorem}
\footnote{
  \citePpc{wicks1986}{898}{has additional $s$ in denominator},
  \citerpgc{shin2008}{293}{0470725648}{(9.67)},
  \citePpc{white2006}{679}{(6)}
  }
\label{thm:estHk}
\label{thm:estHs}
%---------------------------------------
Let $\opS$ be the \structe{system} illustrated in \prefpp{fig:addnoise_LTI}.
Let $\estHkp(\omega)$ be the transfer function estimate defined in \prefpp{def:Hkp}.
%Let \\\indentx$\norm{\Swxx(\omega)}^2\eqd\inprod{\Swxx(\omega)}{\Swxx(\omega)}\eqd\pE ...$
\thmbox{
  \brb{\begin{array}{FMD}
      (1).& There exists $\kappa(\omega)$ such that     &
        \\& $\Swvv(\omega)=\kappa(\omega)\Swuu(\omega)$ & and
    \\(2).& $\fCost(\estHls)=\Swuu(\omega)$             &
  \end{array}}
  \implies
  \brb{\begin{array}{>{\ds}rc>{\ds}l}
    \argmin_{\estH}\fCost(\estH) &=& \estHkp(\omega)
    \\\mc{3}{D}{($\estHkp$ is the ``optimal" estimator for minimizing system noise)}
  \end{array}}
  }
\end{theorem}
\begin{proof}
\begin{enumerate}
  \item Let \label{item:estHk_FG}
        $\begin{array}[t]{rclDD}
             \fF &\eqd& \abs{\estH(\omega)}^2\Swxx(\omega) - \estH(\omega)\Swxy(\omega) - \estH^\ast(\omega)\Swxy^\ast(\omega) + \Swyy(\omega)
               & (numerator in \pref{lem:estHk_Suu})
               & and
           \\\fG &\eqd& \kappa(\omega)+\abs{\estH(\omega)}^2
               & (denominator in \pref{lem:estHk_Suu})
        \end{array}$

  \item lemma $\brp{\pderiv{}{\estH_R}\Swuu}$: \label{ilem:estHk_HR}
    \begin{align*}
      \boxed{0}
        &= \frac{1}{2}\fG^20 = \frac{1}{2}\fG^2\pderiv{}{\estH_R}\Swuu
        && \text{set $\pderiv{}{\estH_R}\Swuu=0$ to find optimum $\estH_R$}
      \\&= \frac{1}{2}\fG^2\pderiv{}{\estH_R}\frac{\fF}{\fG}
        && \text{by \prefp{lem:estHk_Suu}}
      \\&= \frac{1}{2}\fG^2\frac{(\fF'\fG-\fG'\fF)}{\fG^2}
        && \text{by \thme{Quotient Rule}}
      \\&= \frac{1}{2}(\fF'\fG-\fG'\fF)
      \\&= \frac{1}{2}\brs{2\estH_R\Swxx - \Swxy - \Swxy^\ast}\fG - \frac{1}{2}2\estH_R\fF
        && \text{by definition of $\fF$, $\fG$}
        && \text{\xref{item:estHk_FG}}
      \\&= \boxed{\estH_R\Swxx \fG - \fG\Real\Swxy - \estH_R\fF}
    \end{align*}

  \item lemma $\brp{\pderiv{}{\estH_I}\Swuu}$: \label{ilem:estHk_HI}
    \begin{align*}
      \boxed{0}
        &= \frac{1}{2}\fG^20 = \frac{1}{2}\fG^2\pderiv{}{\estH_I}\Swuu
        && \text{set $\pderiv{}{\estH_I}\Swuu=0$ to find optimum $\estH_I$}
      \\&= \frac{1}{2}\fG^20 = \frac{1}{2}\fG^2\pderiv{}{\estH_I}\frac{\fF}{\fG}
        && \text{by \prefp{lem:estHk_Suu}}
      \\&= \frac{1}{2}\fG^2\frac{(\fF'\fG-\fG'\fF)}{\fG^2}
        && \text{by \thme{Quotient Rule}}
      \\&= \frac{1}{2}(\fF'\fG-\fG'\fF)
      \\&= \frac{1}{2}\brs{2\estH_I\Swxx - i\Swxy + i\Swxy^\ast}\fG - \frac{1}{2}2\estH_I\fF
        && \text{by definition of $\fF$, $\fG$}
        && \text{\xref{item:estHk_FG}}
      \\&= \boxed{\estH_I\Swxx \fG + \fG\Imag\Swxy - \estH_I\fF}
    \end{align*}

  \item Solve for $\estH$ \ldots
    \begin{align*}
      0
        &= 0 + i0
         = \frac{1}{2}\fG^20
         + \frac{1}{2}\fG^20
         = \frac{1}{2}\fG^2\pderiv{}{\estH_R}\Swuu
         +i\frac{1}{2}\fG^2\pderiv{}{\estH_I}\Swuu
      \\&= \brs{\estH_R\Swxx \fG - \fG\Real\Swxy - \estH_R\fF}
         +i\brs{\estH_I\Swxx \fG + \fG\Imag\Swxy - \estH_I\fF}
        && \text{by \pref{ilem:estHk_HR} and \pref{ilem:estHk_HI}}
      \\&= \mathrlap{
             \estH\Swxx \fG - \Swxy^\ast \fG - \estH \fF
             \quad\text{because $\Real(z) + i\Imag(z)=z$ and $\Real(z) - i\Imag(z)=z^\ast$}
             }
      \\&= \estH\Swxx \fG - \Swyx \fG - \estH \fF
        && \text{by \prefp{cor:Swxy_sym}}
      \\&= \estH\Swxx\brp{\kappa+\abs{\estH}^2} - \Swyx\brp{\kappa+\abs{\estH}^2}
         - \estH\brp{\abs{\estH}^2\Swxx - \estH\Swxy - \estH^\ast\Swxy^\ast + \Swyy}
        && \text{by $\fF$, $\fG$ defs.}
      \\&= \estH\Swxx\brp{\kappa+\cancelto{}{\abs{\estH}^2}} - \Swyx\brp{\kappa+\abs{\estH}^2}
         - \estH\brp{\cancelto{}{\abs{\estH}^2\Swxx} - \estH\Swxy - \estH^\ast\Swxy^\ast + \Swyy}
      \\&= \kappa\estH\Swxx - \Swyx\brp{\kappa+\abs{\estH}^2}
         + \brp{ \estH^2\Swxy + \abs{\estH}^2\Swxy^\ast - \estH\Swyy}
      \\&= \kappa\estH\Swxx - \kappa\Swyx - \cancelto{}{\Swyx\abs{\estH}^2}
         + \brp{ \estH^2\Swxy + \cancelto{}{\abs{\estH}^2\Swxy^\ast} - \estH\Swyy}
      \\&=  \estH^2\Swxy + \estH\brs{\kappa\Swxx - \Swyy} - \kappa\Swxy^\ast
      \\
      \implies&\boxed{
        \estH = \frac{\brp{\Swyy-\kappa\Swxx} \pm \sqrt{\brp{\Swyy-\kappa\Swxx}^2 + 4\kappa\abs{\Swxy}^2}}
                     {2\Swxy}
      }% Praise the Lord!!!     2019 March 17 Sunday
      && \text{by \thme{Quadratic Equation}}
    \end{align*}
\end{enumerate}
\end{proof}


%20190528%%============================================================================
%20190528%\subsection{Coherence}
%20190528%%============================================================================
%20190528%%=======================================
%20190528%%\subsubsection{Application}
%20190528%%=======================================
%20190528%%Coherence has two basic purposes:
%20190528%%\begin{enume}
%20190528%%  \item The \fncte{coherence} of $\rvx$ and $\rvy$ is a measure of how closely
%20190528%%        $\rvx$ and $\rvy$ are statistically related.
%20190528%%        %That is, it is an indication of how much $\rvx$ and $\rvy$
%20190528%%        %``cohere" or ``stick" together
%20190528%%  \item
%20190528%The \fncte{coherence} of $\rvx$ and $\rvy$ is a measure of how reliable
%20190528%        are the estimates $\estHa$ and $\estHb$ \xxref{def:H1}{def:H2}.
%20190528%        If the coherence is $0.70$ or above, then we can have high confidence that
%20190528%        the estimates $\estHa$ and $\estHb$ are ``good"
%20190528%        estimates.\footnote{\citerpgc{liang2015}{363}{365}{1498702341}{7.4.2\scshape Coherece Function}}
%20190528%%\end{enume}
%20190528%
%20190528%%=======================================
%20190528%%\subsubsection{Definitions}
%20190528%%=======================================
%20190528%%---------------------------------------
%20190528%\begin{definition}
%20190528%\footnote{
%20190528%  \citePp{chen2012}{4699}{(1), (2)},
%20190528%  \citerppgc{liang2015}{363}{365}{1498702341}{7.4.2 Coherence function},
%20190528%  \citerpgc{ewins1986}{131}{0863800173}{$\gamma^2=\ffrac{H_1(\omega)}{H_2(\omega)}$ (3.8)}
%20190528%  }
%20190528%\label{def:Cxy}
%20190528%\label{def:oCxy}
%20190528%%---------------------------------------
%20190528%Let $\opS$ be a \structe{system} with input $\rvx(n)$ and output $\rvy(n)$.
%20190528%\defbox{\begin{array}{MM>{\ds}rc>{\ds}l}
%20190528%  The \fnctd{complex coherence} function &is defined as&
%20190528%    \Cxy(\omega) &\eqd& \frac{\Swxy^\ast(\omega)}{\sqrt{\Swxx(\omega)\Swyy(\omega)}}
%20190528%    \\
%20190528%  The \fnctd{ordinary coherence} function &is defined as&
%20190528%    \oCxy(\omega) &\eqd& \frac{\abs{\Swxy(\omega)}^2}{\Swxx(\omega)\Swyy(\omega)}
%20190528%\end{array}}
%20190528%\end{definition}
%20190528%
