%============================================================================
% Daniel J. Greenhoe
% LaTeX file
%============================================================================
%============================================================================
\subsection{Case study: Dual additive noise}
%============================================================================
%---------------------------------------
\begin{minipage}{\tw-55mm}
\begin{proposition}
\label{prop:dual_addnoise}
%---------------------------------------
Let $\opS$ be the \structe{system} illustrated to the right.
%where $\opT$ is an operator that is \prope{not necessarily linear}.
\end{proposition}
\end{minipage}
\qquad\tbox{\includegraphics{graphics/dual_addnoise.pdf}}
\propbox{
  \brb{\begin{array}{FMD}
      (A).& $\rvx(n)$ and $\rvr(n)$ are \prope{wide sense stationary}      & and
    \\(B).& $\rvx(n)$ and $\rvw(n)$ are \prope{uncorrelated}               & and
    \\(C).& $\rvr(n)$ and $\rvv(n)$ are \prope{uncorrelated}               & and
    \\(D).& $\rvw(n)$ and $\rvv(n)$ are \prope{uncorrelated}               & and
    \\(E).& $\rvv(n)$ and $\rvw(n)$ are \prope{zero-mean}                  &
  \end{array}}
  \implies
  \brb{\begin{array}{rclD}
      \Rsy(m)       &=& \Rrx(m)       & and
    \\\Szsy(z)      &=& \Szrx(z)      & and
    \\\Swsy(\omega) &=& \Swrx(\omega) &
  \end{array}}
  \qquad
  \begin{array}{M}
    for all\\ 
    (1)--(8)
  \end{array}
  }
\\
\begin{proof}
\begin{align*}
  (1).\quad\boxed{\Rsy(m)}
    &\eqd \pE\brs{\rvs(m)\rvy^\ast(0)}
    && \text{by Papoulis' definition of $\Rxy$}
    && \text{\xref{def:Rxym}}
  \\&\eqd \pE\brp{\brs{\rvr(m)+\rvw(m)}\brs{\rvx(0)+\rvv(0)}^\ast}
    && \text{by definition of $\opS$}
  \\&= \mathrlap{
       \pE\brs{\rvr(m)\rvx^\ast(0)}
      +\pE\brs{\rvr(m)\rvv^\ast(0)}
      +\pE\brs{\rvw(m)\rvx^\ast(0)}
      +\pE\brs{\rvw(m)\rvv^\ast(0)}
      }
  \\&= \pE\brs{\rvr(m)\rvx^\ast(0)}
      +\pE\rvr(m)\pE\rvv^\ast(0)
      \\&\qquad
      +\pE\rvw(m)\pE\rvx^\ast(0)
      +\pE\rvw(m)\pE\rvv^\ast(0)
    && \text{by \prope{uncorrelated} hypotheses}
    && \text{(B), (C), and (D)}
  \\&= \pE\brs{\rvr(m)\rvx^\ast(0)}
      +\pE\rvr(m)\cancelto{0}{\pE\rvv^\ast(0)}
      \\&\qquad
      +\cancelto{0}{\pE\rvw(m)}\pE\rvx^\ast(0)
      +\cancelto{0}{\pE\rvw(m)}\pE\rvv^\ast(0)
    && \text{by \prope{zero-mean} hypothesis}
    && \text{(E)}
  \\&\eqd \boxed{\Rrx(m)}
    && \text{by definition of $\Rrx$}
    && \text{\xref{def:Rxym}}
\end{align*}
\begin{align*}
    (2).\quad\Rsy(m)
      &\eqd \pE\brs{\rvs^\ast(0)\rvy(m)}
     &&=\pE\brp{\brs{\rvr(0)+\rvw(0)}^\ast \brs{\rvx(m)+\rvv(m)}}
     &&= \scy \Rrx(m)+\cancelto{0}{\Rrv(m)}+\cancelto{0}{\Rwx(m)}+\cancelto{0}{\Rwv(m)}
     %&&=\scy\pE\brs{\rvr^\ast(0)\rvx(m)}
     %  +\cancelto{0}{\pE\brs{\rvr^\ast(0)\rvv(m)}}
     %  +\cancelto{0}{\pE\brs{\rvw^\ast(0)\rvx(m)}}
     %  +\cancelto{0}{\pE\brs{\rvw^\ast(0)\rvv(m)}}
     &&\eqd\Rrx(m)
    \\
    (3).\quad\Rsy(m)
      &\eqd \pE\brs{\rvs(0)\rvy^\ast(m)}
     &&=\pE\brp{\brs{\rvr(0)+\rvw(0)} \brs{\rvx(m)+\rvv(m)}^\ast}
     &&= \scy \Rrx(m)+\cancelto{0}{\Rrv(m)}+\cancelto{0}{\Rwx(m)}+\cancelto{0}{\Rwv(m)}
     %&&=\scy\pE\brs{\rvr(0)\rvx^\ast(m)}
     %  +\cancelto{0}{\pE\brs{\rvr(0)\rvv^\ast(m)}}
     %  +\cancelto{0}{\pE\brs{\rvw(0)\rvx^\ast(m)}}
     %  +\cancelto{0}{\pE\brs{\rvw(0)\rvv^\ast(m)}}
     &&\eqd\Rrx(m)
    \\
    (4).\quad\Rsy(m)
      &\eqd \pE\brs{\rvs^\ast(m)\rvy(0)}
     &&=\pE\brp{\brs{\rvr(m)+\rvw(m)}^\ast \brs{\rvx(0)+\rvv(0)}}
     &&= \scy \Rrx(m)+\cancelto{0}{\Rrv(m)}+\cancelto{0}{\Rwx(m)}+\cancelto{0}{\Rwv(m)}
     %&&=\scy\pE\brs{\rvr^\ast(m)\rvx(0)}
     %  +\cancelto{0}{\pE\brs{\rvr^\ast(m)\rvv(0)}}
     %  +\cancelto{0}{\pE\brs{\rvw^\ast(m)\rvx(0)}}
     %  +\cancelto{0}{\pE\brs{\rvw^\ast(m)\rvv(0)}}
     &&\eqd\Rrx(m)
    \\
    (5).\quad\Rsy(m)
      &\eqd \pE\brs{\rvs(0)\rvy(m)}
     &&=\pE\brp{\brs{\rvr(0)+\rvw(0)} \brs{\rvx(m)+\rvv(m)}}
     &&= \scy \Rrx(m)+\cancelto{0}{\Rrv(m)}+\cancelto{0}{\Rwx(m)}+\cancelto{0}{\Rwv(m)}
     %&&=\scy\pE\brs{\rvr(0)\rvx(m)}
     %  +\cancelto{0}{\pE\brs{\rvr(0)\rvv(m)}}
     %  +\cancelto{0}{\pE\brs{\rvw(0)\rvx(m)}}
     %  +\cancelto{0}{\pE\brs{\rvw(0)\rvv(m)}}
     &&\eqd\Rrx(m)
    \\
    (6).\quad\Rsy(m)
      &\eqd \pE\brs{\rvs(m)\rvy(0)}
     &&=\pE\brp{\brs{\rvr(m)+\rvw(m)} \brs{\rvx(0)+\rvv(0)}}
     &&= \scy \Rrx(m)+\cancelto{0}{\Rrv(m)}+\cancelto{0}{\Rwx(m)}+\cancelto{0}{\Rwv(m)}
     %&&=\scy\pE\brs{\rvr(m)\rvx(0)}
     %  +\cancelto{0}{\pE\brs{\rvr(m)\rvv(0)}}
     %  +\cancelto{0}{\pE\brs{\rvw(m)\rvx(0)}}
     %  +\cancelto{0}{\pE\brs{\rvw(m)\rvv(0)}}
     &&\eqd\Rrx(m)
    \\
    (7).\quad\Rsy(m)
      &\eqd \pE\brs{\rvs^\ast(0)\rvy^\ast(m)}
     &&=\pE\brp{\brs{\rvr(0)+\rvw(0)}^\ast \brs{\rvx(m)+\rvv(m)}^\ast}
     &&= \scy \Rrx(m)+\cancelto{0}{\Rrv(m)}+\cancelto{0}{\Rwx(m)}+\cancelto{0}{\Rwv(m)}
     %&&=\scy\pE\brs{\rvr(0)^\ast\rvx(m)^\ast}
     %  +\cancelto{0}{\pE\brs{\rvr^\ast(0)\rvv^\ast(m)}}
     %  +\cancelto{0}{\pE\brs{\rvw^\ast(0)\rvx^\ast(m)}}
     %  +\cancelto{0}{\pE\brs{\rvw^\ast(0)\rvv^\ast(m)}}
     &&\eqd\Rrx(m)
    \\
    (8).\quad\Rsy(m)
      &\eqd \pE\brs{\rvs^\ast(m)\rvy^\ast(0)}
     &&=\pE\brp{\brs{\rvr(m)+\rvw(m)}^\ast \brs{\rvx(0)+\rvv(0)}^\ast}
     &&= \scy \Rrx(m)+\cancelto{0}{\Rrv(m)}+\cancelto{0}{\Rwx(m)}+\cancelto{0}{\Rwv(m)}
     %&&=\scy\pE\brs{\rvr(m)^\ast\rvx(0)^\ast}
     %  +\cancelto{0}{\pE\brs{\rvr^\ast(m)\rvv^\ast(0)}}
     %  +\cancelto{0}{\pE\brs{\rvw^\ast(m)\rvx^\ast(0)}}
     %  +\cancelto{0}{\pE\brs{\rvw^\ast(m)\rvv^\ast(0)}}
     &&\eqd\Rrx(m)
\end{align*}
\end{proof}

