%============================================================================
% LaTeX File
% Daniel J. Greenhoe
%============================================================================


%=======================================
\chapter {Pollen Parameterized Wavelets}
%=======================================
David Pollen showed that there are an uncountably infinite number of 
compactly supported scaling functions (and wavelets) available for 
coefficient length 4 and greater.
This is stated in \pref{thm:pollen},
demonstrated in \prefpp{ex:pollen4} and illustrated in \prefpp{fig:pollen4}.
%---------------------------------------
\begin{theorem}[Pollen parameterization theorem]
\label{thm:pollen}
\footnote{
  \citerp{ak}{3}
  }
\index{Pollen parameterization theorem}
\index{theorems!Pollen parameterization theorem}
%---------------------------------------
\thmbox{
\begin{aligned}
  \Zh(z) 
    &= \cwt 
       \left[-1 \quad 1 \right]
       E(z^2)
       \left[\begin{array}{c}-z^{-1}\\ 1 \end{array}\right]
  \\[1ex]
    & \text{where}
  \\[2ex]
  E(z)
    &= \begin{cases}
         U_1 U_2 \dotsm U_{2k}    & \text{for $ h_n $ of length $4k+2$, $k\in\Znn$} \\
         U_1 U_2 \dotsm U_{2k+1}  & \text{for $ h_n $ of length $4k+4$, $k\in\Znn$}
       \end{cases}
  \\
  U(z)
    &= \left[\begin{array}{rr}
         \fu(z)      & \fv(z) \\
        -\fv(z^{-1}) & \fu(z^{-1})
       \end{array}\right]
  \\
  \fu(z) &= \frac{1}{2}\left[(1-\cos\theta)z + (1+\cos\theta) \right]
  \\
  \fv(z) &= \frac{1}{2}\left[(-\sin\theta) + (\sin\theta)z^{-1} \right]
\end{aligned}
}
\end{theorem}
%\begin{proof}
%No proof at this time.
%\end{proof}

%---------------------------------------
\begin{example}[Pollen length-4 scaling coefficients]
\label{ex:pollen4}
\footnote{
  \citerp{ak}{3},
  \citerp{burrus}{66}
  }
%---------------------------------------
\exbox{\begin{array}{r|l}
  n  &  h_n  \\
  \hline
  0  & \ds \frac{\sqrt{2}}{4}(1-\cos\theta+\sin\theta)  \\
  1  & \ds \frac{\sqrt{2}}{4}(1+\cos\theta+\sin\theta)  \\ 
  2  & \ds \frac{\sqrt{2}}{4}(1+\cos\theta-\sin\theta)  \\ 
  3  & \ds \frac{\sqrt{2}}{4}(1-\cos\theta-\sin\theta)
\end{array}}
\end{example}
\begin{proof}
\begin{align*}
  \Zh(z) 
    &= \cwt 
       \left[-1 \quad 1 \right]
       E(z^2)
       \left[\begin{array}{c}-z^{-1}\\ 1 \end{array}\right]
  \\&= \cwt 
       \left[-1 \quad 1 \right]
       U(z^2)
       \left[\begin{array}{c}-z^{-1}\\ 1 \end{array}\right]
  \\&= \cwt 
       \left[-1 \quad 1 \right]
       \left[\begin{array}{rr}
         \fu(z^2)      & \fv(z^2) \\
        -\fv(z^{-2})   & \fu(z^{-2})
       \end{array}\right]
       \left[\begin{array}{c}-z^{-1}\\ 1 \end{array}\right]
  \\&= \cwt 
       \left[-1 \quad 1 \right]
       \left[\begin{array}{cc}
           \frac{1}{2}\left[(1-\cos\theta)z^2 + (1+\cos\theta) \right]
       &   \frac{1}{2}\left[(-\sin\theta) + (\sin\theta)z^{-2} \right]
       \\ -\frac{1}{2}\left[(-\sin\theta) + (\sin\theta)z^{2} \right]
       &   \frac{1}{2}\left[(1-\cos\theta)z^{-2} + (1+\cos\theta) \right]
       \end{array}\right]
       \left[\begin{array}{c}-z^{-1}\\ 1 \end{array}\right]
  \\&= \frac{\sqrt{2}}{4}
       \left[\begin{array}{ll}
          -\left[(1-\cos\theta)z^2 + (1+\cos\theta) \right]
          +\left[(-\sin\theta) + (\sin\theta)z^{2} \right]
       \\ -\left[(-\sin\theta) + (\sin\theta)z^{-2} \right]
          +\left[(1-\cos\theta)z^{-2} + (1+\cos\theta) \right]
       \end{array}\right]^T
       \left[\begin{array}{c}-z^{-1}\\ 1 \end{array}\right]
  \\&= \frac{\sqrt{2}}{4}
       \Bigg[
          (1-\cos\theta)z +(1+\cos\theta)z^{-1}
          -(\sin\theta)z^{-1} +(\sin\theta)z
  \\&\qquad
          + \sin\theta -(\sin\theta)z^{-2}
          +(1-\cos\theta)z^{-2} + (1+\cos\theta)
       \Bigg]
  \\&= \frac{\sqrt{2}}{4}
       \Bigg[
           (1-\cos\theta+\sin\theta)z
          +(1+\cos\theta+\sin\theta)
  \\&\qquad          
          +(1+\cos\theta-\sin\theta)z^{-1}
          +(1-\cos\theta-\sin\theta)z^{-2}
       \Bigg]
\end{align*}
\end{proof}

%\psset{unit=1mm}
%\begin{pspicture}(0,0)(100,100)
%  \psset{%
%    fillstyle=solid,
%    linecolor=black,
%    fillcolor=tan,
%    gridcolor=graph,
%    gridwidth=0.8pt,
%    gridlabels=14pt,
%    subgriddiv=5,
%    %linearc=0.5,
%    %framearc=1,
%    }%
%  %\rput[bl](0,10){\ingr{100\psunit}{100\psunit}{../common/wavelets/p4phi_djg.eps}}%
%  \psline(1,16)(78,4)
%  \rput[t](1,15){$0$}%
%  \rput[t](24,11){$1$}%
%  \rput[t](48,8){$2$}%
%  \rput[t](70,4){$3$}%
%  \psgrid[unit=10\psunit](0,0)(10,10)%
%\end{pspicture}



%\begin{figure}[ht]
%\begin{center}
%\psset{unit=1mm}
%\begin{tabular*}{\textwidth}{@{\extracolsep{\fill}}cc}
%   %\epsfig{file=../common/wavelets/pollen4h.eps, height=7cm, width=7cm}  &
%   %\epsfig{file=../common/wavelets/pollen4g.eps, height=7cm, width=7cm}
%   %\\
%   %$h_n(\theta)$ & $g_n(\theta)$
%   %\\
%   \ingr{\tw/2-5mm}{\tw/2-5mm}{../common/wavelets/graphics/p4phib_djg.eps}  &
%   \ingr{\tw/2-5mm}{\tw/2-5mm}{../common/wavelets/graphics/p4psib_djg.eps}
%   %\ingr{\tw/2-5mm}{\tw/2-5mm}{../common/wavelets/graphics/p4phib_bw_djg.jpg}  &
%   %\ingr{\tw/2-5mm}{\tw/2-5mm}{../common/wavelets/graphics/p4psib_bw_djg.jpg}
%   \\
%   $\fphi(t)$ & $\fpsi(t)$
%\end{tabular*}
%\caption{Pollen scaling and wavelet functions with varying parameter $\theta$
%  \label{fig:pollen4}
%  }
%\end{center}
%\end{figure}

\begin{figure}[ht]
\begin{center}
\psset{unit=1mm}
\begin{tabular*}{\textwidth}{@{\extracolsep{\fill}}cc}
   %\epsfig{file=../common/wavelets/pollen4h.eps, height=7cm, width=7cm}  &
   %\epsfig{file=../common/wavelets/pollen4g.eps, height=7cm, width=7cm}
   %\\
   %$h_n(\theta)$ & $g_n(\theta)$
   %\\
   %\ingr{\tw/2-5mm}{\tw/2-5mm}{../common/wavelets/graphics/p4phib_djg.eps}  &
   %\ingr{\tw/2-5mm}{\tw/2-5mm}{../common/wavelets/graphics/p4psib_djg.eps}
   %\ingr{\tw/2-5mm}{\tw/2-5mm}{../common/wavelets/graphics/p4phib_bw_djg.jpg}  &
   %\ingr{\tw/2-5mm}{\tw/2-5mm}{../common/wavelets/graphics/p4psib_bw_djg.jpg}
   \pgfplotsset{colormap={grayscale}{gray=(0); gray=(0.5)}}%
   \begin{tikzpicture}
     \begin{axis}[
       width=160\psunit,
       height=80\psunit,
       z post scale=2.5,
       xmode=normal,
       ymode=normal,
       zmode=normal,
       xlabel=$\theta$,
       ylabel=$t$,
       zlabel=$\fpsi(t;\theta)$,
       %title="",
       %axis lines=none,
       line width=1pt,
       %colormap/bluered,
       %view={109}{45},
       view={109}{45},
       ]
       %\addplot3[colormap={bw}{gray=(0); gray=(0)},mesh] table[header=false]{plt/p4psi42.dat};
       \addplot3[mesh] table[header=false]{plt/p4psi42.dat};
     \end{axis}
   \end{tikzpicture}
   %&
   %\begin{tikzpicture}
   %  \begin{axis}[
   %    width=160\psunit,
   %    height=80\psunit,
   %    z post scale=2.5,
   %    xmode=normal,
   %    ymode=normal,
   %    zmode=normal,
   %    axis lines=none,
   %    line width=1.5pt,
   %    %colormap/bluered,
   %    view={109}{45},
   %    ]
   %    \addplot3[black,mesh] table[header=false]{plt/p4psi42.dat};
   %  \end{axis}
   %\end{tikzpicture}
   \\
  % $\fphi(t)$ & $\fpsi(t)$
   $\fpsi(t)$
\end{tabular*}
\caption{Pollen length-4 wavelet function with varying parameter $\theta$
  \label{fig:pollen4}
  }
\end{center}
\end{figure}


%\clearpage
%---------------------------------------
\begin{example}[\exmd{Pollen length-6 scaling coefficients}]
\label{ex:pollen6}
\footnote{
  \citerp{burrus}{66},
  \citerp{vidakovic}{95}
  }
%---------------------------------------
Length-6 scaling coefficients have two parameters, 
here designated $\alpha$ and $\beta$.
The scaling coefficients are as follows.
\exbox{
 \begin{array}{c|l}
   n & h_n
   \\ \hline
      0 & \frac{1}{4\sqrt{2}} [(1+\cos(\alpha)+\sin(\alpha))(1-\cos(\beta)-\sin(\beta)) + 2\sin(\beta)\cos(\alpha)] 
   \\ 1 & \frac{1}{4\sqrt{2}}[(1-\cos(\alpha)+\sin(\alpha))(1+\cos(\beta)-\sin(\beta)) - 2\sin(\beta)\cos(\alpha)] 
   \\ 2 & \frac{1}{2\sqrt{2}}[(1+\cos(\alpha-\beta)+\sin(\alpha-\beta)] 
   \\ 3 & \frac{1}{2\sqrt{2}}[(1+\cos(\alpha-\beta)-\sin(\alpha-\beta)] 
   \\ 4 & \frac{1}{ \sqrt{2}} - h(0) - h(2) 
   \\ 5 & \frac{1}{ \sqrt{2}} - h(1) - h(3) 
  \end{array}
}
\end{example}
\if 0
\begin{proof}
\begin{align*}
  \Zh(z) 
    &= \cwt 
       \left[-1 \quad 1 \right]
       E(z^2)
       \left[\begin{array}{c}-z^{-1}\\ 1 \end{array}\right]
  \\&= \cwt 
       \left[-1 \quad 1 \right]
       U_\alpha(z^2)
       U_\beta(z^2)
       \left[\begin{array}{c}-z^{-1}\\ 1 \end{array}\right]
  \\&= \cwt 
       \left[-1 \quad 1 \right]
       \left[\begin{array}{rr}
         \fu_\alpha(z^2)      & \fv_\alpha(z^2) \\
        -\fv_\alpha(z^{-2})   & \fu_\alpha(z^{-2})
       \end{array}\right]
       \left[\begin{array}{rr}
         \fu_\beta(z^2)      & \fv_\beta(z^2) \\
        -\fv_\beta(z^{-2})   & \fu_\beta(z^{-2})
       \end{array}\right]
       \left[\begin{array}{c}-z^{-1}\\ 1 \end{array}\right]
  \\&= \cwt 
       \left[\begin{array}{c@{\qquad}c}
         -\fu_\alpha(z^2)-\fv_\alpha(z^{-2}) &
         -\fv_\alpha(z^2)+\fu_\alpha(z^{-2})
       \end{array}\right]
       \left[\begin{array}{r}
         -z^{-1}\fu_\beta(z^2)+ \fv_\beta(z^2) \\
        z^{-1}\fv_\beta(z^{-2}) +\fu_\beta(z^{-2})
       \end{array}\right]
  \\&= \cwt 
       \left[
         \left(-\fu_\alpha(z^2)        - \fv_\alpha(z^{-2}) \right)
         \left(-z^{-1}\fu_\beta(z^2)   + \fv_\beta(z^2)     \right)+
         \left(-\fv_\alpha(z^2)        + \fu_\alpha(z^{-2}) \right)
         \left(z^{-1}\fv_\beta(z^{-2}) + \fu_\beta(z^{-2})  \right)
       \right]
  \\&= \cwt 
       \Bigg[
         \left(
            z^{-1}\fu_\alpha(z^2)   \fu_\beta(z^2) 
           -      \fu_\alpha(z^2)   \fv_\beta(z^2)
           +z^{-1}\fv_\alpha(z^{-2})\fu_\beta(z^2)
           -      \fv_\alpha(z^{-2})\fv_\beta(z^2)
         \right)
       \\&\qquad+
         \left(
           -z^{-1}\fv_\alpha(z^2)   \fv_\beta(z^{-2})
           -      \fv_\alpha(z^2)   \fu_\beta(z^{-2})
           +z^{-1}\fu_\alpha(z^{-2})\fv_\beta(z^{-2})
           +      \fu_\alpha(z^{-2})\fu_\beta(z^{-2})
         \right)
       \Bigg]
  \\&= \cwt  \frac{1}{4}
       \Bigg[
            z^{-1}\left[(1-\cos\alpha)z^2       + (1+\cos\alpha)     \right]   
                  \left[(1-\cos\beta)z^2        + (1+\cos\beta)      \right] 
       \\&\qquad\qquad
           -      \left[(1-\cos\alpha)z^2       + (1+\cos\alpha)     \right]
                  \left[(-\sin\beta)            + (\sin\beta)z^{-2}  \right]
       \\&\qquad\qquad
           +z^{-1}\left[(-\sin\alpha)           + (\sin\alpha)z^{2}  \right]
                  \left[(1-\cos\beta)z^2        + (1+\cos\beta)      \right]
       \\&\qquad\qquad
           -      \left[(-\sin\alpha)           + (\sin\alpha)z^{2}  \right]
                  \left[(-\sin\beta)            + (\sin\beta)z^{-2}  \right]
       \\&\qquad\qquad
           -z^{-1}\left[(-\sin\alpha)           + (\sin\alpha)z^{-2} \right]
                  \left[(-\sin\beta)            + (\sin\beta)z^{2}   \right]
       \\&\qquad\qquad
           -      \left[(-\sin\alpha)           + (\sin\alpha)z^{-2} \right] 
                  \left[(1-\cos\beta)z^{-2}     + (1+\cos\beta)      \right]
       \\&\qquad\qquad
           +z^{-1}\left[(1-\cos\alpha)z^{-2}    + (1+\cos\alpha)     \right]
                  \frac{1}{2}\left[(-\sin\beta) + (\sin\beta)z^{2}   \right]
       \\&\qquad\qquad
           +      \left[(1-\cos\alpha)z^{-2}    + (1+\cos\alpha)     \right]
                  \left[(1-\cos\beta)z^{-2}     + (1+\cos\beta)      \right]
       \Bigg]
  \\ \vdots
\end{align*}
Proof not yet complete. Current result taken from  \problem \\
\cite[page 66]{burrus}
\end{proof}

\fi


