%============================================================================
% LaTeX File
% Daniel J. Greenhoe
%============================================================================

%======================================
\chapter{Sample Rate Conversion}
\label{app:src}
%======================================


%=======================================
\section{Sample rate conversion}
%=======================================
%---------------------------------------
\begin{theorem}[\thmd{upsampling}]
%\footnote{
%  \citerpgc{strang1996}{101}{0961408871}{Second Nobel Identity}
%  }
\label{thm:upsample}
%---------------------------------------
Let $\seqxZ{x_n}$ and $\seqxZ{y_n}$ be \structe{sequences} \xref{def:seq} 
in $\spllF$ \xref{def:spllF} over a \structe{field} $\F$.
\thmbox{
  y_n = 
  \brb{\begin{array}{lM}
    x_{(n/\xN)} & for $n\mod \xN=0$  \\
    0         & otherwise
  \end{array}}
  \qquad\implies\qquad
  {\Zy(z) = \Zx\brp{z^\xN}}
  }
\end{theorem}
\begin{proof}
\begin{align*}
  \Zy(z)
    &\eqd \sum_{n\in\Z} y_n z^{-n}
    &&    \text{by definition of \fncte{z-transform}}
    &&    \text{\xref{def:opZ}}
  \\&=    \sum_{n\mod\xN=0}   y_n z^{-n} +
          \sum_{n\mod\xN\ne0} y_n z^{-n}
  \\&=    \sum_{n\mod\xN=0} x_{n/\xN} z^{-n} +
          \cancelto{0}{\sum_{n\mod \xN\ne 0} 0 z^{-n}}
    &&    \text{by definition of $\seqn{y_n}$}
  \\&=    \sum_{m\in\Z} x_m z^{-m\xN}
    &&    \text{where $m\eqd n/\xN\,\implies\,n=m\xN$}
  \\&=    \sum_{m\in\Z} x_m \brp{z^\xN}^{-m}
  \\&\eqd \Zx\brp{z^\xN}
    &&    \text{by definition of \fncte{z-transform}}
    &&    \text{\xref{def:opZ}}
\end{align*}
\end{proof}



%---------------------------------------
\begin{theorem}[\thmd{downsampling}]
\index{decimation}
\label{thm:downsample}
%---------------------------------------
Let $\seqxZ{x_n}$ and $\seqxZ{y_n}$ be \structe{sequences} \xref{def:seq} 
in $\spllF$ \xref{def:spllF} over a \structe{field} $\F$.
\thmbox{
  \brb{y_n = x_{(\xN n)}}
  \qquad\implies\qquad
  \brb{\Zy(z)=\frac{1}{\xN}\sum_{m=0}^{\xN-1}\Zx\left( e^{i\frac{2\pi m}{\xN}} z^{\frac{1}{\xN}} \right)}
  }
\end{theorem}
\begin{proof}
\begin{align*}
  \Zy(z)
    &\eqd \sum_{n\in\Z} y_n z^{-n}
    &&    \text{by definition of \fncte{z-transform}}
    &&    \text{\xref{def:opZ}}
  \\&=    \sum_{n\in\Z} x_{(n\xN)} z^{-n}
    &&    \text{by definition of $\seqn{y_n}$}
  \\&=    \sum_{n\in\Z} x_n \Big[ \kdelta_{(n\mod \xN)} \Big] z^{-\frac{n}{\xN}}
  \\&=    \sum_{n\in\Z} x_n \brs{\frac{1}{\xN}\sum_{m=0}^{\xN-1} e^{-i\frac{2\pi nm}{\xN}}} z^{-\frac{n}{\xN}}
    &&    \text{by \thme{Summation around unit circle}}
    &&    \text{\xref{cor:trig_circle}}
  \\&=    \frac{1}{\xN}\sum_{m=0}^{\xN-1} \sum_{n\in\Z} x_n 
                 \brp{e^{i\frac{2\pi m}{\xN}}}^{-n} 
                 \brp{ z^\frac{1}{\xN}}^{-n}
  \\&=    \frac{1}{\xN}\sum_{m=0}^{\xN-1} \sum_{n\in\Z} x_n 
                 \brp{e^{i\frac{2\pi m}{\xN}} z^\frac{1}{\xN}}^{-n} 
  \\&\eqd \frac{1}{\xN}\sum_{m=0}^{\xN-1}\Zx\brp{e^{i\frac{2\pi m}{\xN}} z^\frac{1}{\xN}}
    &&    \text{by definition of \fncte{z-transform}}
    &&    \text{\xref{def:opZ}}
\end{align*}
\end{proof}





