%============================================================================
% LaTeX File
% Daniel Greenhoe
%============================================================================
%=======================================
\chapter{Stromberg Wavelets}
%=======================================
%--------------------------------------
\begin{definition}
\label{def:A0A1}
%--------------------------------------
\defbox{
  \begin{array}{lcl D}
    \setA_0 &\eqd& \setn{\cdots,-\frac{3}{2},-1,-\frac{1}{2},0,1,2,3,\cdots}& and\\
    \setA_1 &\eqd& \setA_0 \setu \setn{\frac{1}{2}}
  \end{array}
  }
\end{definition}

%--------------------------------------
\begin{definition}
\label{def:simple_tent}
%--------------------------------------
The \fnctd{simple tent function} $\fLambda_{\sigma}$ for $\sigma\in\setA_0$ is defined as
\defbox{
  \fLambda_{\sigma}(x) \eqd \brbl{\begin{array}{ll} 
      1-\sigma+x    & \text{for $x\in\intcc{\sigma-1}{\sigma  }$}
    \\1+\sigma-x    & \text{for $x\in\intcc{\sigma  }{\sigma+1}$}
    \\0             & \text{otherwise}
  \end{array}}
  }
\end{definition}

%--------------------------------------
\begin{definition}
\footnote{
  \citerpgc{stromberg1983}{479}{9780534980412}{4. Explicit Description of $\tau$ and $\rho$, $m=0$}
  }
%--------------------------------------
\defbox{
  S(x) \eqd \brbl{\begin{array}{ll} 
        \brs{S(\sigma)-S(\sigma-1)}\brp{x-\sigma}+S(\sigma) & \text{for $x\in\intcc{\sigma-1}{\sigma  }$}
      \\\brs{S(\sigma+1)-S(\sigma)}\brp{x-\sigma}+S(\sigma) & \text{for $x\in\intcc{\sigma  }{\sigma+1}$}
  \end{array}}
  }
\end{definition}

%--------------------------------------
\begin{theorem}
\label{thm:strom_ortho}
\footnote{
  \citeP{stromberg1983},
  \citer{wojtaszczyk1997},
  \citerppgc{jaffard2001}{23}{24}{9780898718119}{{\textsection} 2.5 New Directions of the 1930s: The Franklin System}
  \citer{greenhoe_3964474}
  }
%--------------------------------------
\thmbox{
  0 = \inprod{S(x)}{\fLambda_{\sigma }(x)} = 
    \brbl{\begin{array}{l ll}
      S\brp{\sigma -1}+ 4S\brp{\sigma}+S\brp{\sigma +1}
      &   \text{for $\sigma\in\setn{2,3,4,\ldots}$} 
      \\
      S\brp{0} + 6S\brp{\frac{1}{2}} + 13S\brp{1} + 4S\brp{2}
      &   \text{for $\sigma=1$}
      \\
      2S\brp{-\frac{1}{2}} + 9S\brp{0} + 6S\brp{\frac{1}{2}} + S\brp{1}
      &   \text{for $\sigma=0$}
      \\
      S\brp{\sigma-\frac{1}{2}}+ 4S\brp{\sigma}+S\brp{\sigma+\frac{1}{2}}
      &   \text{for $\sigma\in\setn{\ldots, -\frac{5}{2}, -2, -\frac{3}{2},-1,-\frac{1}{2}}$} 
  \end{array}}
  }
\end{theorem}
\begin{proof}
\begin{enumerate}
  \item lemma: \label{ilem:stromberg_AB} 
    \begin{align*}
        &\int_{x=\sigma-1}^{x=\sigma}   \brs{ (A-B)(x-\sigma)+A           } (1-\sigma+x)    \dx
    \\&= \int_{x=\sigma-1}^{x=\sigma}   \brs{ A(1-\sigma+x) + B(\sigma-x) } (1-\sigma+x)    \dx
    \\&= \int_{x=\sigma-1}^{x=\sigma}  A\brs{ x^2 + 2x(1-\sigma)        + (1-\sigma)^2    } 
                                     + B\brs{-x^2 +  x(\sigma+\sigma-1) + \sigma(1-\sigma)} \dx
    \\&= \brs{ A\brs{ \frac{1}{3}x^3 +             x^2(1-\sigma ) + x(1-\sigma)^2    } 
             + B\brs{-\frac{1}{3}x^3 + \frac{1}{2} x^2(2\sigma-1) + x\sigma(1-\sigma)}
             }_{x=\sigma-1}^{x=\sigma}
    \\&= A\brs{ \frac{1}{3}\brp{\sigma^3-\brp{\sigma^3-3\sigma^2+3\sigma-1}} +            \brp{\sigma^2-\brp{\sigma^2-2\sigma+1}}(1-\sigma ) + (1-\sigma)^2\brp{\sigma-(\sigma-1)} } 
    \\&+ B\brs{-\frac{1}{3}\brp{\sigma^3-\brp{\sigma^3-3\sigma^2+3\sigma-1}} + \frac{1}{2}\brp{\sigma^2-\brp{\sigma^2-2\sigma+1}}(2\sigma-1) + \sigma(1-\sigma)                    }
    \\&= A\brs{ \brp{\sigma^2 - \sigma + \frac{1}{3} } +            (2\sigma-1)(1-\sigma ) + (-\sigma+1)^2     }
       + B\brs{-\brp{\sigma^2 - \sigma + \frac{1}{3} } + \frac{1}{2}(2\sigma-1)(2\sigma-1) + \sigma(-\sigma+1) }
    \\&= A\brs{\sigma^2( 1-2+1) + \sigma(-1+2+1-2) + \brp{ \frac{1}{3}-1+1}}
       + B\brs{\sigma^2(-1+2-1) + \sigma( 1-1-1+1) + \brp{-\frac{1}{3}+\frac{1}{2}}}
    \\&= \boxed{\frac{1}{3}A + \frac{1}{6}B}
    \end{align*}

  \item lemma: \label{ilem:stromberg_CA} 
    \begin{align*}
        &\int_{x=\sigma}^{x=\sigma+1}   \brs{ (C-A)(x-\sigma)+C           } (1+\sigma-x)    \dx
    \\&= \int_{x=\sigma}^{x=\sigma+1}   \brs{ C(1-\sigma+x) + A(\sigma-x) } (1+\sigma-x)    \dx
    \\&= \int_{x=\sigma}^{x=\sigma+1}  C\brs{-x^2 +  x(\sigma+\sigma+1) + \sigma(-\sigma-1)    } 
                                     + A\brs{ x^2 +  x(-\sigma-1-1-\sigma) + (1+\sigma)^2} \dx
    \\&= \brs{ C\brs{-\frac{1}{3}x^3 + \frac{1}{2} x^2(2\sigma+1) - x\sigma(\sigma+1)}
              +A\brs{ \frac{1}{3}x^3 -             x^2( \sigma+1) + x(\sigma+1)^2    } 
             }_{x=\sigma}^{x=\sigma+1}
    \\&= C\brs{-\frac{1}{3}\brp{\brp{\sigma^3+3\sigma^2+3\sigma+1}-\sigma^3} + \frac{1}{2}\brp{\brp{\sigma^2+2\sigma+1}-\sigma^2}(2\sigma+1) - \sigma(\sigma+1) }
    \\&+ A\brs{ \frac{1}{3}\brp{\brp{\sigma^3+3\sigma^2+3\sigma+1}-\sigma^3} -            \brp{\brp{\sigma^2+2\sigma+1}-\sigma^2}( \sigma+1) + (\sigma+1)^2     } 
    \\&= C\brs{-\sigma^2 + \sigma - \frac{1}{3} + \frac{1}{2}(2\sigma+1)(2\sigma+1) - \sigma^2 -\sigma }
       + A\brs{ \sigma^2 + \sigma + \frac{1}{3} - (2\sigma+1)( \sigma+1) + \sigma^2 + 2\sigma + 1      }
    \\&= C\brs{\sigma^2(-1+2-1) + \sigma(-1+1+1-1) + \brp{-\frac{1}{3}+\frac{1}{2}}}
       + A\brs{\sigma^2( 1-2+1) + \sigma( 1-2-1+2) + \brp{ \frac{1}{3}-1+1}}
    \\&= \boxed{\frac{1}{6}C + \frac{1}{3}A}
    \end{align*}

  \item definitions: Let $A\eqd S(\sigma)$, $B\eqd S(\sigma-1)$, and $C\eqd S(\sigma+1)$. \label{idef:stromberg_ABC}
  \item Finish proof\ldots
    \begin{align*}
      \inprod{S(x)}{\fLambda_\sigma(x)}
        &= \int_{x\in\mathbb{R}}S(x)\fLambda_\sigma(x)\dx
        && \text{by definition of $\inprod{x}{y}$}
      \\&= \int_{x=\sigma-1}^{x=\sigma+1}S(x)\fLambda_\sigma(x)\dx
        && \text{because support of $\fLambda_\sigma$ is $\intcc{\sigma-1}{\sigma+1}$}
      \\&= \int_{x=\sigma-1}^{x=\sigma}S(x)\fLambda_\sigma(x)\dx
         + \int_{x=\sigma}^{x=\sigma+1}S(x)\fLambda_\sigma(x)\dx
      \\&\eqd \int_{x=\sigma-1}^{x=\sigma  } \brs{ (A-B)(x-\sigma)+A } (1-\sigma+x) \dx
         + \int_{x=\sigma  }^{x=\sigma+1} \brs{ (C-A)(x-\sigma)+C } (1+\sigma-x) \dx
        && \text{by \pref{idef:stromberg_ABC}}
      \\&= \frac{1}{3}A + \frac{1}{6}B + \frac{1}{6}C + \frac{1}{3}A
        && \text{by \pref{ilem:stromberg_AB} and \pref{ilem:stromberg_CA}}
      \\&= \frac{1}{6}\brs{B + 4A + C}
      \\&\eqd \boxed{\frac{1}{6}\brs{S(\sigma-1) + 4S(\sigma) + S(\sigma+1)}}
        && \text{by \pref{idef:stromberg_ABC}}
    \end{align*}
\end{enumerate}
\end{proof}


