%============================================================================
% Daniel J. Greenhoe
% GNU Ocatave file
% 1st order low pass filter design
%============================================================================
%=======================================
%\chapter{Coefficient Calculation}
%=======================================
%----------------------------------------------------------------------------
\section{2nd Order \propb{low-pass} calculation---polynomial form}
%----------------------------------------------------------------------------
%---------------------------------------
% problem statement
%---------------------------------------
 \vfill
\begin{align*}
  \boxed{\Fh(\omega)}
    &= \brlr{\Zh(z)}_{z=e^{i\omega}}
  \\&= \brlr{G\brs{\frac{\brp{1+z^{-1}}^2}
                        {1 + az^{-1} + bz^{-2}}}}_{z=e^{i\omega}}
  \\&= \boxed{\brlr{
         G\brs{\frac{1 + 2z^{-1} +  z^{-2}}
                    {1 + az^{-1} + bz^{-2}}
              }
                   }_{z=e^{i\omega}}
             }
\end{align*}
\vfill
We need 3 equations to solve for the 3 unkowns $G$, $a$, and $b$
\vfill 
%---------------------------------------
Equation 1: Gain=1 at DC
%---------------------------------------
\vfill
\begin{align*}
  1 &= \abs{\Fh(0)}
  \\&= \brlr{\Zh(z)}_{z=e^{i\omega},\,\omega=0}
  \\&= \brlr{G\brs{\frac{\brp{1+z^{-1}}^2}
                      {1 + az^{-1} + bz^{-2}}}}_{z=1}
  \\&= \frac{4G}{1 + a + b}
   %&& \text{(see \prefpo{equ:trickdc})}
  \\&\implies \boxed{G = \frac{a + b + 1}{4}}
\end{align*}
\vfill 

%---------------------------------------
Equation 2: Gain = $\sfrac{1}{2}$ at corner frequency
%---------------------------------------
\begin{align*}
  \boxed{\abs{\Fh(\omega)}^2}
    &= \abs{\Zh(z)}^2_{z=e^{i\omega}}
     = \abs{G\brs{\frac{\brp{1+z^{-1}}^2}
                      {1 + az^{-1} + bz^{-2}}}}^2_{z=e^{i\omega}}
  \\&=     {\frac{\ds\sum_{n=0}^{2}b_n^2 + 2\sum_{n=0}^{2}\ds\sum_{m=n+1}^{2} b_n b_m \cos\brs{\omega(n-m)}}
                 {\ds\sum_{n=0}^{2}a_n^2 + 2\sum_{n=0}^{2}\ds\sum_{m=n+1}^{2} a_n a_m \cos\brs{\omega(n-m)}}}
    %\qquad\text{(see \prefpo{equ:mr})}
  \\&=     G^2\brs{\frac{\ds\brp{1^2+2^2+1^2} + 2\brs{2\cos(\omega) + \cos(2\omega) + 2\cos(\omega)}}
                    {\ds\brp{1^2+a^2+b^2} + 2b\cos(2\omega) + 2a(b+1)\cos(\omega) + (1+a^2+b^2)}}
  \\&={G^2\brs{\frac{\ds2 \cos(2\omega) + 8\cos(\omega) + 6}
                    {\ds2b\cos(2\omega) + 2a(b+1)\cos(\omega) + (a^2+b^2+1)}}}
\end{align*}
$\ds\boxed{
  G^2\brs{\frac{\ds2 \cos(2\omega_c) + 8\cos(\omega_c) + 6}
                    {\ds2b\cos(2\omega_c) + 2a(b+1)\cos(\omega_c) + (a^2+b^2+1)}}
  = \frac{1}{2}
  }$
\vfill 

%---------------------------------------
Equation 3: For more smoothness in passband, set 2nd derivative to 0:
%---------------------------------------
{\begin{align*}
  0 &= \ddwddw\abs{\Fh(\omega)}^2_{\omega=0}
  \\&= \ddwddw G^2 \brs{\frac{\ff(\omega)}
                             {\fg(\omega)}
                       }_{\omega=0}
  \\&= \ddw    G^2 \brs{\frac{\ff'\fg + \ff \fg'}
                             {\fg^2}
                       }_{\omega=0}
    && \text{by \thme{product rule}}
  \\&=         G^2 \brs{\frac{(\ff''\fg + \ff'\fg' - \ff'\fg' -\ff\fg'')\fg^2 - (\ff'\fg - \ff\fg')(2\fg\fg')}
                             {\fg^4}
                       }_{\omega=0}
  \\&=         G^2 \brs{\frac{\ff''\fg -\ff\fg''}
                             {\fg^2}
                       }_{\omega=0}
     \qquad \implies \boxed{\brlr{\ff''\fg = \ff\fg''}_{\omega=0}}
\end{align*}
\ldots because $\ff'(0) = \fg'(0) = 0$ %(see \prefpo{equ:mrflat})
 
{ \begin{align*}
  &\implies \mcom{\brs{-8\cos(2\omega)-8\cos(\omega)}}
                   { $\ff''$}
                    \mcom{\brs{2b\cos(2\omega)+2a(b+1)\cos(\omega)+(a^2+b^2+1)}}
                         { $\fg$}
              \\&\qquad= \brlr{\mcom{\brs{2\cos(2\omega) + 8\cos(\omega) + 6}}
                                    { $\ff$}
                  + \mcom{\brs{-8b\cos(2\omega)-2a(b+1)\cos(\omega)}}
                         { $\fg''$}
                   }_{\omega=0} 
  \\&\implies \brs{-8-8}        \brs{2b+2a(b+1)+(a^2+b^2+1)}
                = \brs{2 + 8 + 6} + \brs{-8b-2a(b+1)}
  \\&\implies 16\brp{a^2+b^2 +2ab + 2a + 2b + 1} = 2ab + 2a + 8b + 16
  \\&\implies 16a^2+ 16b^2 +30ab + 30a + 24b = 0
  \\&\implies \boxed{8a^2+ 8b^2 +15ab + 15a + 12b = 0}
\end{align*}}




%---------------------------------------
\begin{example}2nd order \propb{low-pass} with corner frequency $\omega_c=\frac{2}{3}\pi$
%---------------------------------------
{ \begin{align*}
  1&= \Fh(0) = \brlr{\Zh(z)}_{z=e^{i0}} = \frac{G(1+1)^2}{1+a+b} &&\implies \boxed{4G = a + b + 1}
  \\\\
  \frac{1}{2} 
    &= \abs{G\brs{\frac{\brp{1+z^{-1}}^2}
                  {1 + az^{-1} + bz^{-2}}}}^2_{z=e^{i2\pi/3}}
   &&=     G^2\brs{\frac{\ds2 \cos(4\pi/3) + 8\cos(2\pi/3) + 6}
                    {\ds2b\cos(4\pi/3) + 2a(b+1)\cos(2\pi/3) + (a^2+b^2+1)}}
  \\&= \mathrlap{G^2\brs{\frac{\ds-\sqrt{3} - 4 + 6}
                    {\ds-b\sqrt{3} - a(b+1) + (a^2+b^2+1)}}}
  \\&=       \frac{\ds G^2\brp{2 -\sqrt{3}}}
                  {\ds a^2+b^2-ab-a-\sqrt{3}b}
    &&\implies \boxed{2\brp{2 -\sqrt{3}}G^2 = a^2+b^2-ab-a-\sqrt{3}b}
\end{align*}}

 
 We can combine the previous two \fbox{boxed} equations to eliminate $G$
\\
{ \begin{align*}
  0 &= 8\times0
  \\&= 8\brs{(1-c)a^2 + (1-c)b^2 - (2c+1)ab - (2c+1)a - (2c-\sqrt{3})b -3c }
    \quad\text{where $\ds c=\frac{2-\sqrt{3}}{8}$}
  \\&=8\brs{ 
       \brp{\frac{6+\sqrt{3}}{8}}a^2 
      +\brp{\frac{6+\sqrt{3}}{8}}b^2 
      -\brp{\frac{6-\sqrt{3}}{4}}ab 
      -\brp{\frac{6-\sqrt{3}}{4}}a
      -\brp{\frac{2-3\sqrt{3}}{4}}b
      -\brp{\frac{6-3\sqrt{3}}{8}}c
      }
  \\&= \brp{6+\sqrt{3}}a^2 
      +\brp{6+\sqrt{3}}b^2 
      -\brp{12-2\sqrt{3}}ab 
      -\brp{12-2\sqrt{3}}a
      -\brp{4-6\sqrt{3}}b
      -\brp{6-3\sqrt{3}}c
\end{align*}

Combined equations:\\
$\ds\boxed{
   \brp{6+\sqrt{3}}a^2 
      +\brp{6+\sqrt{3}}b^2 
      -\brp{12-2\sqrt{3}}ab 
      -\brp{12-2\sqrt{3}}a
      -\brp{4-6\sqrt{3}}b
      -\brp{6-3\sqrt{3}}c
  = 0}$



2nd derivative equation:\\
\boxed{8a^2+ 8b^2 +15ab + 15a + 12b = 0}
}
\end{example}