%============================================================================
% XeLaTeX File
% Daniel J. Greenhoe
%============================================================================

%=======================================
\chapter{Magnitude characteristics of z-filters}
%=======================================

%---------------------------------------
\begin{remark}
%---------------------------------------
The frequency response of $\Zh(z)$ \propb{repeats} every $2\pi$ (every $F_s$).
\end{remark}
\begin{proof}
\begin{align*}
  \Fh(\omega-2\pi n)
    &\eqd \brlr{\Zh(z)}_{z=e^{i(\omega-2\pi n)}}
    && \text{by definition of $\Fh(\omega)$}
  \\&\eqd \brlr{\sum_{m\in\Z} \fx[m] z^{-m}}_{z=e^{i(\omega-2\pi n)}}
    &&\text{by definition of $\opZ$}
  \\&= \sum_{m\in\Z} \fx[m] e^{-i\omega m}\cancelto{1}{e^{-i2\pi nm}}
  \\&\eqd \brlr{\sum_{m\in\Z} \fx[m] z^{-m}}_{z=e^{i\omega}}
  \\&\eqd \brlr{\Zh(z)}_{z=e^{i\omega}}
    &&\text{by definition of $\opZ$}
  \\&\eqd \Fh(\omega)
    && \text{by definition of $\Fh(\omega)$}
\end{align*}
\end{proof}

%---------------------------------------
\begin{remark}
%---------------------------------------
If the coefficients are \propb{real}, then the magnitude response (MR) is \propb{symmetric}
\end{remark}
\begin{proof}
\begin{align*}
  \abs{\Fh(-\omega)}
    &\eqd \abs{\Zh(z)}_{z=e^{-i\omega}}
   &&\eqd \abs{\sum_{m\in\Z} \fx[m] z^{-m}}_{z=e^{-i\omega}}
  \\&= \abs{\sum_{m\in\Z} \fx[m] e^{i\omega m}}
   &&= \abs{\brp{\sum_{m\in\Z} \fx^\ast[m] e^{-i\omega m}}^\ast}
  \\&= \mcom{\abs{\brp{\sum_{m\in\Z} \fx[m] e^{-i\omega m}}^\ast}}
            { if $x[m]$ is \prope{real}}
   &&= \abs{\sum_{m\in\Z} \fx[m] e^{-i\omega m}}
  \\&\eqd \abs{\Zh(z)}_{z=e^{-i\omega}}
   &&\eqd \abs{\Fh(\omega)}
\end{align*}
\end{proof}

%%---------------------------------------
%
%\# 2: If the coefficients are \propb{real}, then the MR is \propb{symmetric}
%%---------------------------------------
%{\begin{align*}
%  \boxed{\abs{H(\omega)}^2}
%    &= \abs{H(z)}^2_{z=e^{i\omega}}
%     = \brlr{H(z)H^\ast(z)}_{z=e^{i\omega}}
%     = \brlr{
%         \brp{\frac{\ds\sum_{n=0}^{\xN}b_nz^{-n}}
%                   {\ds\sum_{n=0}^{\xN}a_nz^{-n}}}
%         \brp{\frac{\ds\sum_{n=0}^{\xN}b_nz^{-n}}
%                   {\ds\sum_{n=0}^{\xN}a_nz^{-n}}}^\ast
%         }_{z=e^{i\omega}}
%  \\&= \brp{\frac{\ds\sum_{n=0}^{\xN}b_ne^{-i\omega n}}
%                 {\ds\sum_{n=0}^{\xN}a_ne^{-i\omega n}}}  
%       \brp{\frac{\ds\sum_{n=0}^{\xN}b_ne^{-i\omega n}}
%                 {\ds\sum_{n=0}^{\xN}a_ne^{-i\omega n}}}^\ast
%     = \brp{\frac{\ds\sum_{n=0}^{\xN}b_ne^{-i(-\omega) n}}
%                 {\ds\sum_{n=0}^{\xN}a_ne^{-i(-\omega) n}}}  
%       \brp{\frac{\ds\sum_{n=0}^{\xN}b_ne^{-i(-\omega) n}}
%                 {\ds\sum_{n=0}^{\xN}a_ne^{-i(-\omega) n}}}^\ast
%  \\&= H(-\omega)H^\ast(-\omega)
%     = \boxed{\abs{H(-\omega)}^2}
%\end{align*}}

%---------------------------------------
%\# 3: MR is flat at $\omega=0$ and $\omega=\pi$ 
%---------------------------------------

%---------------------------------------
\begin{lemma}
\label{lem:aacos}
%---------------------------------------
\lembox{
  \sum_{n=0}^{\xN}\ds\sum_{m=0}^{\xN} a_n a_m e^{-i\omega(n-m)}
    =\sum_{n=0}^{\xN}\abs{a_n}^2 + 2\sum_{n=0}^{\xN}\ds\sum_{m=n+1}^{\xN} \Re\brs{a_n a_m^\ast} \cos\brs{\omega(n-m)}
  }
\end{lemma}

%---------------------------------------
\begin{example}
This example graphically illustrates \prefpp{lem:aacos} for the case $\xN=4$.
%---------------------------------------
\begin{align*}
  \sum_{n=0}^{4}\ds\sum_{m=0}^{4} a_n a_m e^{-i\omega(n-m)}
    &= \brp{\begin{array}{|c||*{5}{>{\ds}c|}}
           \hline          &{\ccg}$m=0$                 &{\ccg}$m=1$                 &{\ccg}$m=2$                 &{\ccg}$m=3$                 &{\ccg}$m=4$
         \\\hline
           \hline\ccg$n=0$ &{\ccc}a_0 a_0^\ast               &      a_0 a_1^\ast e^{+i \omega} &      a_0 a_2^\ast e^{+i2\omega} &      a_0 a_3^\ast e^{+i3\omega} &      a_0 a_4^\ast e^{+i4\omega} 
         \\\hline\ccg$n=1$ &      a_1 a_0^\ast e^{-i \omega} &{\ccc}a_1 a_1^\ast               &      a_1 a_2^\ast e^{+i \omega} &      a_1 a_3^\ast e^{+i2\omega} &      a_1 a_4^\ast e^{+i3\omega} 
         \\\hline\ccg$n=2$ &      a_2 a_0^\ast e^{-i2\omega} &      a_2 a_1^\ast e^{-i \omega} &{\ccc}a_2 a_2^\ast               &      a_2 a_3^\ast e^{+i \omega} &      a_2 a_4^\ast e^{+i2\omega} 
         \\\hline\ccg$n=3$ &      a_3 a_0^\ast e^{-i3\omega} &      a_3 a_1^\ast e^{-i2\omega} &      a_3 a_2^\ast e^{-i \omega} &{\ccc}a_3 a_3^\ast               &      a_3 a_4^\ast e^{+i \omega} 
         \\\hline\ccg$n=4$ &      a_4 a_0^\ast e^{-i4\omega} &      a_4 a_1^\ast e^{-i3\omega} &      a_4 a_2^\ast e^{-i2\omega} &      a_4 a_3^\ast e^{-i \omega} &{\ccc}a_4 a_4^\ast                  
         \\\hline
       \end{array}}
  \\&=  \sum_{n=0}^{4}a_n a_n^\ast
     + 2\sum_{n=0}^{4}\ds\sum_{m=n+1}^{4} \brs{\brp{a_n a_m^\ast e^{i\omega}} + \brp{a_n^\ast a_m e^{-i\omega}}}
  \\&=  \sum_{n=0}^{4}a_n a_n^\ast
     + 2\sum_{n=0}^{4}\ds\sum_{m=n+1}^{4} \brs{\brp{a_n a_m^\ast e^{i\omega}} + \brp{a_n a_m^\ast e^{i\omega}}^\ast}
  \\&=  \sum_{n=0}^{4}a_n a_n^\ast
     +  \sum_{n=0}^{4}\ds\sum_{m=n+1}^{4} 2\Re\brs{\brp{a_n a_m^\ast e^{i\omega}}}
  \\&=  \sum_{n=0}^{4}\abs{a_n}^2 
     + 2\sum_{n=0}^{4}\ds\sum_{m=n+1}^{4}  \Re\brs{a_n a_m^\ast} \Re\brs{e^{i\omega(n-m)}}
  \\&=  \sum_{n=0}^{4}\abs{a_n}^2 
     + 2\sum_{n=0}^{4}\ds\sum_{m=n+1}^{4}  \Re\brs{a_n a_m^\ast} \cos\brs{\omega(n-m)}
\end{align*}
\end{example}

%---------------------------------------
\begin{lemma}
\label{lem:qzcos}
%---------------------------------------
\lembox{
  \brb{\Zq(z) \eqd \sum_{n=0}^{\xN} a_n z^{-n}}
  \quad\implies\quad
  \brb{\abs{\Fq(\omega)}^2
    = \sum_{n=0}^{\xN}\abs{a_n}^2 + 2\sum_{n=0}^{\xN} \sum_{m=n+1}^{\xN} a_n a_m^\ast \cos\brs{\omega(n-m)}
    }
  }
\end{lemma}
\begin{proof}
\begin{align*}
  \boxed{\abs{\Fq(\omega)}^2}
    &= \brs{\abs{\Zq(z)}^2}_{z=e^{i\omega}}
  \\&= \brs{\Zq(z)\Zq^\ast(z)}_{z=e^{i\omega}}
  \\&= \brs{\brp{\sum_{n=0}^{\xN} a_n      z^{-n}}
            \brp{\sum_{n=0}^{\xN} a_n^\ast z^{ n}}}_{z=e^{i\omega}}
  \\&= \brs{\sum_{m=0}^{\xN}\sum_{n=0}^{\xN} a_m a_n^\ast z^{n-m}}_{z=e^{i\omega}}
  \\&= \sum_{m=0}^{\xN}\sum_{n=0}^{\xN} a_m a_n^\ast e^{i\omega(n-m)}
  \\&= \sum_{n=0}^{\xN}a_n^2 + 2\sum_{n=0}^{\xN}\ds\sum_{m=n+1}^{\xN} a_n a_m \cos\brs{\omega(n-m)}
    && \text{by \prefp{lem:aacos}}
\end{align*}
\end{proof}

%---------------------------------------
\begin{theorem}
%---------------------------------------
\thmbox{
  \abs{\Fh(\omega)}^2
    =\frac{\ds\sum_{n=0}^{\xN}b_n^2 + 2\sum_{n=0}^{\xN}\ds\sum_{m=n+1}^{\xN} b_n b_m \cos\brs{\omega(n-m)}}
          {\ds\sum_{n=0}^{\xN}a_n^2 + 2\sum_{n=0}^{\xN}\ds\sum_{m=n+1}^{\xN} a_n a_m \cos\brs{\omega(n-m)}}
  }
\end{theorem}
\begin{proof}
\begin{align*}
  \boxed{\abs{\Fh(\omega)}^2}
    &= \abs{\Zh(z)}^2_{z=e^{i\omega}}
  \\&= \brs{\Zh(z)\Zh^\ast(z)}_{z=e^{i\omega}}
  \\&= \abs{\frac{\ds\sum_{n=0}^{\xN}b_n z^{-n}}{\ds\sum_{n=0}^{\xN}a_n z^{-n}}}^2_{z=e^{i\omega}}  
  \\&=\boxed{\frac{\ds\sum_{n=0}^{\xN}b_n^2 + 2\sum_{n=0}^{\xN}\ds\sum_{m=n+1}^{\xN} b_n b_m \cos\brs{\omega(n-m)}}
                  {\ds\sum_{n=0}^{\xN}a_n^2 + 2\sum_{n=0}^{\xN}\ds\sum_{m=n+1}^{\xN} a_n a_m \cos\brs{\omega(n-m)}}}
    && \text{by \prefp{lem:qzcos}}
\end{align*}
\end{proof}


%---------------------------------------
\begin{theorem}
%---------------------------------------
\thmbox{\ddw\abs{\Fh(\omega)}^2_{\omega=0} = 0}
\end{theorem}
\begin{proof}
\begin{align*}
  \ddw\abs{\Zh(z)}^2_{z=e^{i\omega},\omega=0}  
    &= \ddw\brs{\Zh(z)\Zh^\ast(z)}_{z=e^{i\omega},\omega=0}
  \\&= \ddw\brs{\frac{\ds\sum_{n=0}^{\xN}b_n^2 + 2\sum_{n=0}^{\xN}\ds\sum_{m=n}^{\xN} b_n b_m \cos\brs{\omega(n-m)}}
                 {\ds\sum_{n=0}^{\xN}a_n^2 + 2\sum_{n=0}^{\xN}\ds\sum_{m=n}^{\xN} a_n a_m \cos\brs{\omega(n-m)}}}_{\omega=0}
  \\&\eqd \ddw\brs{\frac{\ff(\omega)}{\fg(\omega)}}_{\omega=0}
  \\&= \brs{\frac{\ff'(\omega)\fg(\omega) - \ff(\omega)\fg'(\omega)}{\fg^2(\omega)}}_{\omega=0}
    \qquad\text{by the \thmb{Quotient Rule}}
  \\&= 0
    \qquad\brp{\begin{array}[t]{MMM}
      because & $\ddw$constant$=0$                   & and \\
              & $\ddw\cos(k\omega)=-\sin(k\omega)=0$ & at $\omega=0,\,\pi$
    \end{array}}
\end{align*}
\end{proof}

%---------------------------------------
\begin{remark}
%---------------------------------------
Moments and derivatives are related:
\begin{align*}
  \ddw\brlr{\Fh(\omega)}_{\omega=0}
    &\eqd \ddw\brlr{\Zh(z)}_{z=e^{i\omega},\,\omega=0}
   &&\eqd \ddw\brlr{\sum_{m\in\Z} \fx[m] z^{-m}}_{z=e^{i\omega},\,\omega=0}
  \\&= \ddw\brlr{\sum_{m\in\Z} \fx[m] e^{-i\omega m}}_{\omega=0}
  \\&= \brlr{\sum_{m\in\Z} \fx[m] \ddw e^{-i\omega m}}_{\omega=0}
  \\&= \brlr{\sum_{m\in\Z} \fx[m] (-im) e^{-i\omega m}}_{\omega=0}
  \\&= -i \mcom{\sum_{m\in\Z} m \fx[m]}
               { 1st moment}
\end{align*}
\end{remark}
