$\newcommand{\ds}{\displaystyle}$
$\newcommand{\mean}{\mu}$
$\newcommand{\popvar}{\sigma^2}$
$\newcommand{\cmom}{\mu}$
$\newcommand{\meanest}{\hat{\mean}}$
$\newcommand{\seqn}[1]{\left\{#1\right\}}$
$\newcommand{\rvx}{x}$
$\newcommand{\xN}{N}$
$\newcommand{\eqd}{\triangleq}$
$\newcommand{\brp}[1]{{\left(#1\right)}}$
$\newcommand{\brs}[1]{{\left[#1\right]}}$
$\newcommand{\brl}[1]{{\left.#1\right|}}$
$\newcommand{\moment}{M}$
$\newcommand{\momest}{\hat{\moment}}$
$\newcommand{\meanest}{\hat{\mean}}$
$\newcommand{\cmomest}{\hat{\cmom}}$
$\newcommand{\varest}{\hat{\var}}$
$\newcommand{\popvarest}{\hat{\popvar}}$
$\newcommand{\samvarest}{\hat{s^2}}$
$\newcommand{\mcom}[2]{{\displaystyle\underbrace{\displaystyle#1}_{\text{#2}}}}$
$\newcommand{\indentx}{\ensuremath{\mbox{}\qquad}}$
$\newcommand{\bcoef}[2]{{#1\choose#2}}$

An alternative solution using central moments $\ldots$

(1) Estimated Mean in recursive form
------------------------------------
Define $\meanest_{n}\eqd 0$ for $n=0$.
\begin{align*}
  \boxed{\mcom{\meanest_{n}}{new}}
    &\eqd \frac{1}{n} \sum_{k=1}^{n} \rvx_k
    && \text{by definition of average}
  \\&= \frac{1}{n}\rvx_n + \frac{1}{n} \sum_{k=1}^{n-1} \rvx_k
  \\&= \frac{1}{n}\rvx_n + \frac{n-1}{n}\brs{\frac{1}{n-1} \sum_{k=1}^{n-1} \rvx_k }
  \\&\eqd \frac{1}{n}\rvx_n + \frac{n-1}{n}\meanest_{n-1}
    && \text{by definition of $\meanest$}
  \\&= \frac{1}{n}\rvx_n + \meanest_{n-1} - \frac{1}{n}\meanest_{n-1}
  \\&= \boxed{\mcom{\meanest_{n-1}}{old} + \mcom{\frac{1}{n}}{weight} \mcom{\brs{\rvx_n - \meanest_{n-1}}}{error}}
    && \text{for $n>0$}
\end{align*}

**Example**:
Let $X \eqd \seqn{1,2,3,4,5}$ be a finite sequence of numbers.
The *average* of $X$ is $\ds
  \boxed{\meanest} \eqd \frac{1}{\xN}\sum_{n=1}^\xN x_n
                   =    \frac{1}{5}\brp{1+2+3+4+5}
                   =    \frac{15}{5}
                   =    \boxed{3}
$.  
Using the recursive method of (1) yields the same result:
$\begin{array}{l|rclcl clcl cl}
  n=1 & \meanest_1 &=& \meanest_0   &+& \frac{1}{1}\brp{ \rvx_1 - \meanest_0 }
                   &=& 0            &+&          1 \brp{ 1      - 0          }
                   &=& 1\\
  n=2 & \meanest_2 &=& \meanest_1   &+& \frac{1}{2}\brp{ \rvx_2 - \meanest_1 }
                   &=& 1            &+& \frac{1}{2}\brp{ 2      - 1          }
                   &=& \frac{3}{2} \\
  n=3 & \meanest_3 &=& \meanest_2   &+& \frac{1}{3}\brp{ \rvx_3 - \meanest_2 }
                   &=& \frac{3}{2}  &+& \frac{1}{3}\brp{ 3      - \frac{3}{2}}
                   &=& 2           \\
  n=4 & \meanest_4 &=& \meanest_3   &+& \frac{1}{4}\brp{ \rvx_4 - \meanest_3 }
                   &=& 2            &+& \frac{1}{4}\brp{ 4      - 2          }
                   &=& \frac{5}{2} \\
  n=5 & \boxed{\meanest_5} &=& \meanest_4   &+& \frac{1}{5}\brp{ \rvx_5 - \meanest_4 }
                   &=& \frac{5}{2}  &+& \frac{1}{5}\brp{ 5      - \frac{5}{2}}
                   &=& \boxed{3}
\end{array}$


References: 
[Candy (2009) pages 11-12](http://books.google.com/books?vid=ISBN9780470430576&pg=PA11),
[Candy (2016) pages 12-13](http://books.google.com/books?vid=ISBN9781119125457&pg=PA12)

(2) Estimated order-$p$ Central Moment in recursive form
--------------------------------------------------------
\begin{align*}
  \boxed{\cmomest_{p,n}}
    &\eqd \frac{1}{n} \sum_{k=1}^{n} \brp{ \rvx_k - \meanest_n }^p
          \qquad\text{by definition of order-$p$ central moment}
  \\&=    \frac{1}{n} \sum_{k=1}^{n} \brs{ \rvx_k - \meanest_{n-1} - \frac{1}{n}\brp{ \rvx_n - \meanest_{n-1} } }^p
  \\&=    \frac{1}{n} \sum_{k=1}^{n} \sum_{m=0}^p \bcoef{p}{m} \brs{ \rvx_k - \meanest_{n-1} }^{p-m} \brs{ - \frac{1}{n}\brp{ \rvx_n - \meanest_{n-1} } }^m
          \qquad\text{by Binomial Theorem}
  \\&=    \frac{1}{n} \sum_{m=0}^p \bcoef{p}{m}  \brs{ - \frac{1}{n}\brp{ \rvx_n - \meanest_{n-1} } }^m  \sum_{k=1}^{n} \brs{ \rvx_k - \meanest_{n-1} }^{p-m}
  \\&=    \frac{1}{n} \sum_{m=0}^p \bcoef{p}{m}  \brs{ - \frac{1}{n}\brp{ \rvx_n - \meanest_{n-1} } }^m
                      \brs{(n-1)\mcom{\frac{1}{n-1}\sum_{k=1}^{n-1} \brp{ \rvx_k - \meanest_{n-1} }^{p-m}}{$\cmomest_{p-m,n-1}$} + \brp{ \rvx_n - \meanest_{n-1} }^{p-m} }
  \\&\eqd \boxed{
          \frac{1}{n} \sum_{m=1}^n \bcoef{p}{m}
          \brs{ -\frac{1}{n}\brp{\rvx_n-\meanest_{n-1}} }^m
          \brs{ (n-1) \cmomest_{p-m,n-1} + \brp{ \rvx_n - \meanest_{n-1} }^{p-m} }}
\end{align*}

(3) A couple useful lemmas
--------------------------
\begin{align*}
  \boxed{\cmomest_0}
    &\eqd \frac{1}{n} \sum_{k=1}^{n} \brp{ \rvx_k - \meanest_n }^0
   &&=  \frac{1}{n} \sum_{k=1}^{n} 1
   &&=  \frac{n}{n}
   &&=  \boxed{1}
  \\
  \boxed{\cmomest_1}
    &\eqd \frac{1}{n} \sum_{k=1}^{n} \brp{ \rvx_k - \meanest_n }^1
   &&= \mcom{\brs{\frac{1}{n} \sum_{k=1}^{n} \rvx_k}}{$\meanest_n$} - \brs{\frac{1}{n} \sum_{k=1}^{n} \meanest_n }
   &&= \meanest_n - \frac{n}{n} \meanest_n
   &&= \boxed{0}
\end{align*}

(4) Estimated 2nd Central Moment in recursive form
--------------------------------------------------
\begin{align*}
\boxed{\cmomest_{2,n}}
  &= \frac{1}{n}\sum_{m=1}^n \bcoef{2}{m} \brs{ -\frac{1}{n}\brp{\rvx_n-\meanest_{n-1}} }^m \brs{ (n-1) \cmomest_{2-m,n-1} + \brp{ \rvx_n - \meanest_{n-1} }^{2-m} }
     \qquad\text{by (2)}
  \\&= \frac{1}{n}\mcom{\bcoef{2}{0}}{1} 1 \brs{ (n-1) \cmomest_{2,n-1} + \brp{ \rvx_n - \meanest_{n-1} }^{2} } 
     + \frac{1}{n}\mcom{\bcoef{2}{1}}{2} \brs{ -\frac{1}{n}\brp{\rvx_n-\meanest_{n-1}} }\brs{ (n-1) \mcom{\cmomest_{1,n-1}}{0 by (3)} + \brp{ \rvx_n - \meanest_{n-1} } } 
     + \frac{1}{n}\mcom{\bcoef{2}{2}}{1} \brs{ -\frac{1}{n}\brp{\rvx_n-\meanest_{n-1}} }^2 \brs{ (n-1) \mcom{\cmomest_{0,n-1}}{1 by (3)} + 1 }
  \\&= \brs{\frac{n-1}{n} \cmomest_{2,n-1}
     + \frac{1}{n}\brp{ \rvx_n - \meanest_{n-1} }^2}
     -\frac{2}{n^2} \brp{ \rvx_n - \meanest_{n-1} }^2 +\frac{1}{n^2} \brp{ \rvx_n - \meanest_{n-1} }^2 \brs{ (n-1) + 1 }
  \\&= \brs{\frac{n-1}{n}}\cmomest_{2,n-1} + \brs{ \frac{1}{n} - \frac{2}{n^2} + \frac{1}{n^2} } \brp{ \rvx_n - \meanest_{n-1} }^2
  \\&= \boxed{\brs{\frac{n-1}{n}}\mcom{\cmomest_{2,n-1}}{previous} 
     + \brs{ \frac{n-1}{n^2} } \mcom{\brp{ \rvx_n - \meanest_{n-1} }^2}{error squared}}
\end{align*}

**Example**:
Let $X \eqd \seqn{1,2,3,4,5}$ be a finite sequence of numbers.
The 2nd central moment estimate of $X$ is
\begin{align*}
  \boxed{\cmomest_2} &\eqd \frac{1}{\xN}\sum_{n=1}^\xN \brp{x_n -\meanest}^2
                     =    \frac{1}{5}\brs{ (1-3)^2 + (2-3)^2 + (3-3)^2 + (4-3)^2 + (5-3)^2 }
                  \\&=    \frac{1}{5}\brs{ 4 + 1 + 0 + 1 + 4 }
                     =    \frac{10}{5}
                     =    \boxed{2}
\end{align*}
Using the recursive method of (4) yields the same result:  
$\begin{array}{l|rclcl clcl clcl cl}
  n=1 & \cmomest_{2,1} &=& \frac{1-1}{1}\cmomest_{2,0} &+& \frac{1-1}{1^2}\brp{ \rvx_1 - \meanest_0  }^2
                       &=& 0            \cmomest_{2,0} &+& 0              \brp{ 1      - \meanest_0  }^2
                       &=& 0\\
  n=2 & \cmomest_{2,2} &=& \frac{2-1}{2}\cmomest_{2,1} &+& \frac{2-1}{2^2}\brp{ \rvx_2 - \meanest_1  }^2
                       &=& \frac{1}{2}  0              &+& \frac{1}{4}    \brp{ 2      - 1           }^2
                       &=& \frac{1}{4}\\
  n=3 & \cmomest_{2,3} &=& \frac{3-1}{3}\cmomest_{2,2} &+& \frac{3-1}{3^2}\brp{ \rvx_3 - \meanest_2  }^2
                       &=& \frac{2}{3}  \frac{1}{4}    &+& \frac{2}{9}    \brp{ 3      - \frac{3}{2} }^2
                       &=& \frac{2}{3}\\
  n=4 & \cmomest_{2,4} &=& \frac{4-1}{4}\cmomest_{2,3} &+& \frac{4-1}{4^2}\brp{ \rvx_4 - \meanest_3  }^2
                       &=& \frac{3}{4}  \cdot 1        &+& \frac{3}{16}   \brp{ 4      - 2           }^2
                       &=& \frac{5}{4}\\
  n=5 & \boxed{\cmomest_{2,5}} &=& \frac{5-1}{5}\cmomest_{2,4} &+& \frac{5-1}{5^2}\brp{ \rvx_5 - \meanest_4  }^2
                       &=& \frac{4}{5}  \frac{5}{4}    &+& \frac{4}{25}   \brp{ 5      - \frac{5}{2} }^2
                       &=& \boxed{2}
\end{array}$

(5) Population Variance Estimation
----------------------------------
This follows directly from (4) in any of several forms (use square root function to get associated Standard Deviation estimates):
\begin{align*}
  \popvarest_n
    &\eqd \cmomest_{2,n}
   &&= \brs{\frac{n-1}{n}}\popvarest_{2,n-1} + \brs{ \frac{n-1}{n^2} } \brp{ \rvx_n - \meanest_{n-1} }^2
   \\
  \popvarest_{m+1}
    &\eqd \cmomest_{2,m+1}
   &&=    \brs{\frac{m}{m+1}}\popvarest_{2,m} + \brs{ \frac{m}{(m+1)^2} } \brp{ \rvx_{m+1} - \meanest_{m} }^2
   &&     \text{where $m\eqd n-1\implies n=m+1$}
\end{align*}

(6) Sample Variance Estimation
------------------------------
This follows from (5) and *[Bessel's Correction](https://mathworld.wolfram.com/BesselsCorrection.html)* (use square root function to get associated Standard Deviation estimates):
\begin{align*}
  \samvarest_n
    &\eqd \mcom{\brs{\frac{n}{n-1}}}{Bessel's Correction} \cmomest_{2,n}
     \implies \cmomest_{2,n}   = \brs{\frac{n-1}{n}}\samvarest_n
     \implies \boxed{\cmomest_{2,n-1} = \brs{\frac{n-2}{n-1}}\samvarest_{n-1}}
    &&\text{[Lemma-(5)]}
    \\\\
  \boxed{\samvarest_n}
    &\eqd \mcom{\brs{\frac{n}{n-1}}}{Bessel's Correction} \cmomest_{2,n}
  \\&=  \brs{\frac{n}{n-1}}\brs{\frac{n-1}{n}}\cmomest_{2,n-1} + \brs{\frac{n}{n-1}}\brs{ \frac{n-1}{n^2} } \brp{ \rvx_n - \meanest_{n-1} }^2
    &&  \text{by (4)}
  \\&=  \cmomest_{2,n-1} + \brs{ \frac{1}{n} } \brp{ \rvx_n - \meanest_{n-1} }^2
  \\&=  \boxed{\brs{\frac{n-2}{n-1}}\samvarest_{2,n-1} + \brs{ \frac{1}{n} } \brp{ \rvx_n - \meanest_{n-1} }^2}
    &&  \text{by [Lemma-(5)]}
    \\\\
  \samvarest_{m+1}
    &=  \brs{\frac{m-1}{m}}\samvarest_{2,m} + \brs{ \frac{1}{m+1} } \brp{ \rvx_{m+1} - \meanest_{m} }^2
    && \text{where $m\eqd n-1\implies n=m+1$}
\end{align*}
