%============================================================================
% Daniel J. Greenhoe
% LaTeX file
%============================================================================
%============================================================================
\subsection{Case study: Additive noise}
%============================================================================
%---------------------------------------
\begin{minipage}{\tw-55mm}
\begin{proposition}
\label{prop:xvy}
%---------------------------------------
Let $\opS$ be the \structe{system} illustrated to the right,
where $\opT$ is an operator that is \prope{not necessarily linear}.
\end{proposition}
\end{minipage}
\hfill\tbox{\includegraphics{graphics/sys_xvy.pdf}}
\propbox{
  \brb{\begin{array}{@{\hspace{2pt}}FMMD}
      (A).& $\rvx(n)$ is                & \prope{WSS}          & and 
    \\(B).& $\rvx(n)$ and $\rvv(n)$ are & \prope{uncorrelated} & and
    \\(C).& $\rvv(n)$ is                & \prope{zero-mean}
  \end{array}}
  \implies
  \brb{\begin{array}{rclD}
    %  \Ryv(m) &=&           \Rvv(m)           & and
       \Rxy(m)       &=& \Rxx(m)                       & and
     \\\Szxy(z)      &=& \Szxx(z)                      & and
     \\\Swxy(\omega) &=& \Swxx(\omega)                 & and
     \\\Ryy(m)       &=& \Rxx(m)       + \Szvv(z)      & and
     \\\Szyy(z)      &=& \Szxx(z)      + \Szvv(z)      & and
     \\\Swyy(\omega) &=& \Swxx(\omega) + \Swvv(\omega) &
    %\\\Rxx(m) &=& \mc{2}{l}{\Ryy(m) + \Rvv(m) - 2\Real\Ryv(m)}
  \end{array}}
  \quad
  \begin{array}{M}
    for all\\
    (1)--(8)
  \end{array}
  }
\\
\begin{proof}
\begin{align*}
  (1).\quad\Rxy(m)
    &\eqd \pE\brs{\rvx(m)\rvy^\ast(0)}
    && \text{by (A) and Papoulis' definition of $\Rxy$}
    && \text{\xref{def:Rxym}}
  \\&\eqd \pE\brp{\rvx(m)\brs{\rvx(0)+\rvv(0)}^\ast}
    && \text{by definition of $\rvy$}
  \\&= \pE\brs{\rvx(m)\rvx^\ast(0)} + \pE\brs{\rvx(m)\rvv^\ast(0)}
    && \text{by \prope{linearity} of $\pE$}
    && \text{\xref{prop:pE_linop}}
  \\&= \pE\brs{\rvx(m)\rvx^\ast(0)} + \pE\brs{\rvx(m)} \pE\brs{\rvv^\ast(0)}
    && \text{by \prope{uncorrelated} hypothesis}
    && \text{(B)}
  \\&= \pE\brs{\rvx(m)\rvx^\ast(0)} + \pE\brs{\rvx(m)} \cancelto{0}{\pE\brs{\rvv^\ast(0)}}
    && \text{by \prope{zero-mean} hypothesis}
    && \text{(C)}
  \\&= \Rxx(m)
    && \text{by definition of $\Rxx$}
    && \text{\xref{def:Rxxm}}
\end{align*}
%
\begin{align*}
  \Ryy(m)
    &\eqd \pE\brs{\rvy(m)\rvy^\ast(0)}
    && \text{by (A) and Papoulis' definition of $\Ryy$}
    %&& \text{\xref{def:Rxym}}
  \\&\eqd \pE\brs{(\rvx(m)+\rvv(m))(\rvx(0)+\rvv(0))^\ast}
    && \text{by definition of $\rvy$}
  \\&= \pE\brs{\rvx(m)\rvx^\ast(0)}
     + \pE\brs{\rvx(m)\rvv^\ast(0)}
     + \pE\brs{\rvv(m)\rvx^\ast(0)}
     + \pE\brs{\rvv(m)\rvv^\ast(0)}
  \\&= \pE\brs{\rvx(m)\rvx^\ast(0)}
     + \pE{\rvx(m)\pE\rvv^\ast(0)}
     + \pE{\rvv(m)\pE\rvx^\ast(0)}
     + \pE\brs{\rvv(m)\rvv^\ast(0)}
    &&\text{by \prope{uncorrelated} hypothesis (B)}
  \\&= \pE\brs{\rvx(m)\rvx^\ast(0)}
     + \pE\rvx(m)\cancelto{0}{\pE\rvv^\ast(0)}
     + \cancelto{0}{\pE\rvv(m)}\pE\rvx^\ast(0)
     + \pE\brs{\rvv(m)\rvv^\ast(0)}
    &&\text{by \prope{zero-mean} hypothesis (C)}
  \\&= \Rxx(m) + \Rvv(m)
    && \text{by Papoulis' definition of $\Rxx$}
    %&& \text{\xref{def:Rxxm}}
\end{align*}

\begin{align*}
    (2).\quad\Rxy(m)
       &\eqd \pE\brs{\rvx^\ast(0)\rvy(m)}
      &&\eqd \pE\brp{\rvx^\ast(0)\brs{\rvx(m)+\rvv(m)}}
      &&=    \pE\brs{\rvx^\ast(0)\rvx(m)} + \pE\brs{\rvx^\ast(0)                       \rvv(m)}
     %&&=    \pE\brs{\rvx^\ast(0)\rvx(m)} + \pE\brs{\rvx^\ast(0)} \pE\brs{             \rvv(m)}
     %&&=    \pE\brs{\rvx^\ast(0)\rvx(m)} + \pE\brs{\rvx^\ast(0)} \cancelto{0}{\pE\brs{\rvv(m)}}
      &&=    \Rxx(m)
     \\
    (3).\quad\Rxy(m)
       &\eqd \pE\brs{\rvx(0)\rvy^\ast(m)}
      &&\eqd \pE\brp{\rvx(0)\brs{\rvx(m)+\rvv(m)}^\ast}
      &&=    \pE\brs{\rvx(0)\rvx^\ast(m)} + \pE\brs{\rvx(0)                       \rvv^\ast(m)}
     %&&=    \pE\brs{\rvx(0)\rvx^\ast(m)} + \pE\brs{\rvx(0)} \pE\brs{             \rvv^\ast(m)}
     %&&=    \pE\brs{\rvx(0)\rvx^\ast(m)} + \pE\brs{\rvx(0)} \cancelto{0}{\pE\brs{\rvv^\ast(m)}}
      &&=    \Rxx(m)
     \\
    (4).\quad\Rxy(m)
      &\eqd \pE\brs{\rvx^\ast(m)\rvy(0)}
      &&\eqd \pE\brp{\rvx^\ast(m)\brs{\rvx(0)+\rvv(0)}}
      &&=    \pE\brs{\rvx^\ast(m)\rvx(0)} + \pE\brs{\rvx^\ast(m)                       \rvv(0)}
     %&&=    \pE\brs{\rvx^\ast(m)\rvx(0)} + \pE\brs{\rvx^\ast(m)} \pE\brs{             \rvv(0)}
     %&&=    \pE\brs{\rvx^\ast(m)\rvx(0)} + \pE\brs{\rvx^\ast(m)} \cancelto{0}{\pE\brs{\rvv(0)}}
      &&=    \Rxx(m)
     \\
    (5).\quad\Rxy(m)
      &\eqd \pE\brs{\rvx(0)\rvy(m)}
      &&\eqd \pE\brp{\rvx(0)\brs{\rvx(m)+\rvv(m)}}
      &&=    \pE\brs{\rvx(0)\rvx(m)} + \pE\brs{\rvx(0)                       \rvv(m)}
     %&&=    \pE\brs{\rvx(0)\rvx(m)} + \pE\brs{\rvx(0)} \pE\brs{             \rvv(m)}
     %&&=    \pE\brs{\rvx(0)\rvx(m)} + \pE\brs{\rvx(0)} \cancelto{0}{\pE\brs{\rvv(m)}}
      &&=    \Rxx(m)
     \\
    (6).\quad\Rxy(m)
      &\eqd \pE\brs{\rvx(m)\rvy(0)}
      &&\eqd \pE\brp{\rvx(m)\brs{\rvx(0)+\rvv(0)}}
      &&=    \pE\brs{\rvx(m)\rvx(0)} + \pE\brs{\rvx(m)                       \rvv(0)}
     %&&=    \pE\brs{\rvx(m)\rvx(0)} + \pE\brs{\rvx(m)} \pE\brs{             \rvv(0)}
     %&&=    \pE\brs{\rvx(m)\rvx(0)} + \pE\brs{\rvx(m)} \cancelto{m}{\pE\brs{\rvv(0)}}
      &&=    \Rxx(0)
    \\
    (7).\quad\Rxy(m)
      &\eqd \pE\brs{\rvx^\ast(0)\rvy^\ast(m)}
      &&\eqd \pE\brp{\rvx^\ast(0)\brs{\rvx^\ast(m)+\rvv^\ast(m)}}
      &&=    \pE\brs{\rvx^\ast(0)\rvx(m)} + \pE\brs{\rvx^\ast(0)                       \rvv^\ast(m)}
     %&&=    \pE\brs{\rvx^\ast(0)\rvx(m)} + \pE\brs{\rvx^\ast(0)} \pE\brs{             \rvv^\ast(m)}
     %&&=    \pE\brs{\rvx^\ast(0)\rvx(m)} + \pE\brs{\rvx^\ast(0)} \cancelto{0}{\pE\brs{\rvv^\ast(m)}}
      &&=    \Rxx(m)
    \\
    (8).\quad\Rxy(m)
      &\eqd \pE\brs{\rvx^\ast(m)\rvy^\ast(0)}
      &&\eqd \pE\brp{\rvx^\ast(m)\brs{\rvx^\ast(0)+\rvv^\ast(0)}}
      &&=    \pE\brs{\rvx^\ast(m)\rvx(0)} + \pE\brs{\rvx^\ast(m)                       \rvv^\ast(0)}
     %&&=    \pE\brs{\rvx^\ast(m)\rvx(0)} + \pE\brs{\rvx^\ast(m)} \pE\brs{             \rvv^\ast(0)}
     %&&=    \pE\brs{\rvx^\ast(m)\rvx(0)} + \pE\brs{\rvx^\ast(m)} \cancelto{m}{\pE\brs{\rvv^\ast(0)}}
      &&=    \Rxx(m)
  \end{align*}
  \begin{align*}
    (2).\quad\Ryy(m)
        &\eqd \pE\brs{\rvy^\ast(0)\rvy(m)}
       &&\eqd \pE\brp{\brs{\rvx(0)+\rvv(0)}^\ast\brs{\rvx(m)+\rvv(m)}}
       &&= \scy \Rxx(m) + \cancelto{0}{\Rxv(m)} + \cancelto{0}{\Rvx(m)} + \Rvv(m)
       &&=    \Rxx(m)                                                 + \Rvv(m)
    \\
    (3).\quad\Ryy(m)
        &\eqd \pE\brs{\rvy(0)\rvy^\ast(m)}
       &&\eqd \pE\brp{\brs{\rvx(0)+\rvv(0)}\brs{\rvx(m)+\rvv(m)}^\ast}
       &&= \scy \Rxx(m) + \cancelto{0}{\Rxv(m)} + \cancelto{0}{\Rvx(m)} + \Rvv(m)
       &&=    \Rxx(m)                                                 + \Rvv(m)
    \\
    (4).\quad\Ryy(m)
        &\eqd \pE\brs{\rvy^\ast(m)\rvy(0)}
       &&\eqd \pE\brp{\brs{\rvx(m)+\rvv(m)}^\ast\brs{\rvx(0)+\rvv(0)}}
       &&= \scy \Rxx(m) + \cancelto{0}{\Rxv(m)} + \cancelto{0}{\Rvx(m)} + \Rvv(m)
       &&=    \Rxx(m)                                                 + \Rvv(m)
    \\
    (5).\quad\Ryy(m)
        &\eqd \pE\brs{\rvy(0)\rvy(m)}
       &&\eqd \pE\brp{\brs{\rvx(0)+\rvv(0)}\brs{\rvx(m)+\rvv(m)}}
       &&= \scy \Rxx(m) + \cancelto{0}{\Rxv(m)} + \cancelto{0}{\Rvx(m)} + \Rvv(m)
       &&=    \Rxx(m)                                                 + \Rvv(m)
    \\
    (6).\quad\Ryy(m)
        &\eqd \pE\brs{\rvy(m)\rvy(0)}
       &&\eqd \pE\brp{\brs{\rvx(m)+\rvv(m)}\brs{\rvx(0)+\rvv(0)}}
       &&= \scy \Rxx(m) + \cancelto{0}{\Rxv(m)} + \cancelto{0}{\Rvx(m)} + \Rvv(m)
       &&=    \Rxx(m)                                                 + \Rvv(m)
    \\
    (7).\quad\Ryy(m)
       &\eqd \pE\brs{\rvy^\ast(0)\rvy^\ast(m)}
       &&\eqd \pE\brp{\brs{\rvx(0)+\rvv(0)}^\ast\brs{\rvx(m)+\rvv(m)}^\ast}
       &&= \scy \Rxx(m) + \cancelto{0}{\Rxv(m)} + \cancelto{0}{\Rvx(m)} + \Rvv(m)
       &&=    \Rxx(m)                                                 + \Rvv(m)
    \\
    (8).\quad\Ryy(m)
       &\eqd \pE\brs{\rvy^\ast(m)\rvy^\ast(0)}
       &&\eqd \pE\brp{\brs{\rvx(m)+\rvv(m)}^\ast\brs{\rvx(0)+\rvv(0)}^\ast}
       &&= \scy \Rxx(m) + \cancelto{0}{\Rxv(m)} + \cancelto{0}{\Rvx(m)} + \Rvv(m)
       &&=    \Rxx(m)                                                 + \Rvv(m)
\end{align*}
\end{proof}

